ccomp-simd/common/Values.v
@@ -21,6 +21,8 @@ Require Import AST.
 Require Import Integers.
 Require Import Floats.
 
+Require Import ArchiVec.
+
 Definition block : Type := positive.
 Definition eq_block := peq.
 
@@ -31,15 +33,17 @@ Definition eq_block := peq.
   to this address;
 - the [Vundef] value denoting an arbitrary bit pattern, such as the
   value of an uninitialized variable.
+- vector data (arch. dependent)
 *)
 
 Inductive val: Type :=
   | Vundef: val
   | Vint: int -> val
   | Vlong: int64 -> val
-  | V128: int128 -> val
   | Vfloat: float -> val
-  | Vptr: block -> int -> val.
+  | Vsingle: float32 -> val
+  | Vptr: block -> ptrofs -> val
+  | Vvec: forall t, vec_typ_sem t -> val.
 
 Definition Vzero: val := Vint Int.zero.
 Definition Vone: val := Vint Int.one.
@@ -47,6 +51,12 @@ Definition Vmone: val := Vint Int.mone.
 
 Definition Vtrue: val := Vint Int.one.
 Definition Vfalse: val := Vint Int.zero.
+
+Definition Vnullptr :=
+  if Archi.ptr64 then Vlong Int64.zero else Vint Int.zero.
+
+Definition Vptrofs (n: ptrofs) :=
+  if Archi.ptr64 then Vlong (Ptrofs.to_int64 n) else Vint (Ptrofs.to_int n).
 
 (** * Operations over values *)
 
@@ -56,15 +66,50 @@ Definition Vfalse: val := Vint Int.zero.
 
 Module Val.
 
+Definition eq (x y: val): {x=y} + {x<>y}.
+Proof.
+destruct x; destruct y; auto; try (right; discriminate).
+- elim (Int.eq_dec i i0); intro E;
+  [left; rewrite E| right; intro A; elim E; inversion_clear A];
+  reflexivity. 
+- elim (Int64.eq_dec i i0); intro E;
+  [left; rewrite E| right; intro A; elim E; inversion_clear A];
+  reflexivity. 
+- elim (Float.eq_dec f f0); intro E;
+  [left; rewrite E| right; intro A; elim E; inversion_clear A];
+  reflexivity. 
+- elim (Float32.eq_dec f f0); intro E;
+  [left; rewrite E| right; intro A; elim E; inversion_clear A];
+  reflexivity. 
+- elim (eq_block b b0); intro E;
+  [rewrite E| right; intro A; elim E; inversion_clear A;
+   reflexivity].
+  clear E; elim (Ptrofs.eq_dec i i0); intros E;
+  [left; rewrite E| right; intro A; elim E; inversion_clear A];
+  reflexivity. 
+- elim (Archi.vec_typ_eq t t0); intro E;
+  [ generalize v; rewrite E; intro v1
+  | right; intro A; elim E; inversion_clear A; reflexivity].
+  clear v E; elim (ArchiVec.vec_eq t0 v1 v0); intros E;
+  [left; rewrite E; reflexivity|].
+  right; intro A; elim E; inversion A.
+  apply (Eqdep_dec.inj_pair2_eq_dec); [exact Archi.vec_typ_eq|]; auto.
+Defined.
+Global Opaque eq.
+
 Definition has_type (v: val) (t: typ) : Prop :=
   match v, t with
   | Vundef, _ => True
   | Vint _, Tint => True
   | Vlong _, Tlong => True
-  | V128 _, T128 => True
   | Vfloat _, Tfloat => True
-  | Vfloat f, Tsingle => Float.is_single f
-  | Vptr _ _, Tint => True
+  | Vsingle _, Tsingle => True
+  | Vptr _ _, Tint => Archi.ptr64 = false
+  | Vptr _ _, Tlong => Archi.ptr64 = true
+  | (Vint _ | Vsingle _), Tany32 => True
+  | Vptr _ _, Tany32 => Archi.ptr64 = false
+  | (Vint _ | Vsingle _ | Vlong _ | Vfloat _ | Vptr _ _), Tany64 => True
+  | Vvec t1 _, Tvec t2 => t1=t2
   | _, _ => False
   end.
 
@@ -81,12 +126,28 @@ Definition has_opttype (v: val) (ot: option typ) : Prop :=
   | Some t => has_type v t
   end.
 
+Lemma Vptr_has_type:
+  forall b ofs, has_type (Vptr b ofs) Tptr.
+Proof.
+  intros. unfold Tptr, has_type; destruct Archi.ptr64; reflexivity.
+Qed.
+
+Lemma Vnullptr_has_type:
+  has_type Vnullptr Tptr.
+Proof.
+  unfold has_type, Vnullptr, Tptr; destruct Archi.ptr64; reflexivity.
+Qed.
+
 Lemma has_subtype:
   forall ty1 ty2 v,
   subtype ty1 ty2 = true -> has_type v ty1 -> has_type v ty2.
 Proof.
-  intros. destruct ty1; destruct ty2; simpl in H; discriminate || assumption || idtac.
-  unfold has_type in *. destruct v; auto. 
+  intros. destruct ty1; destruct ty2; simpl in H;
+  try discriminate H || assumption;
+  try (unfold has_type in *; destruct v; auto; contradiction).
+  revert H; elim (Archi.vec_typ_eq v0 v1); simpl.
+   intros -> _; assumption.
+  intros _ H; discriminate H.
 Qed.
 
 Lemma has_subtype_list:
@@ -98,15 +159,45 @@ Proof.
   simpl in *. InvBooleans. destruct H0. split; auto. eapply has_subtype; eauto.
 Qed.
 
-(** Truth values.  Pointers and non-zero integers are treated as [True].
+Definition has_type_dec (v: val) (t: typ) : { has_type v t } + { ~ has_type v t }.
+Proof.
+  unfold has_type; destruct v.
+- auto.
+- destruct t; auto.
+- destruct t; auto.
+- destruct t; auto.
+- destruct t; auto.
+- destruct t; auto.
+  apply bool_dec.
+  apply bool_dec.
+- destruct t; auto.
+  apply Archi.vec_typ_eq.   
+Defined.
+
+Definition has_rettype (v: val) (r: rettype) : Prop :=
+  match r, v with
+  | Tret t, _ => has_type v t
+  | Tint8signed, Vint n => n = Int.sign_ext 8 n
+  | Tint8unsigned, Vint n => n = Int.zero_ext 8 n
+  | Tint16signed, Vint n => n = Int.sign_ext 16 n
+  | Tint16unsigned, Vint n => n = Int.zero_ext 16 n
+  | _, Vundef => True
+  | _, _ => False
+  end.
+
+Lemma has_proj_rettype: forall v r,
+  has_rettype v r -> has_type v (proj_rettype r).
+Proof.
+  destruct r; simpl; intros; auto; destruct v; try contradiction; exact I.
+Qed.
+
+(** Truth values.  Non-zero integers are treated as [True].
   The integer 0 (also used to represent the null pointer) is [False].
-  [Vundef] and floats are neither true nor false. *)
+  Other values are neither true nor false. *)
 
 Inductive bool_of_val: val -> bool -> Prop :=
   | bool_of_val_int:
-      forall n, bool_of_val (Vint n) (negb (Int.eq n Int.zero))
-  | bool_of_val_ptr:
-      forall b ofs, bool_of_val (Vptr b ofs) true.
+      forall n, bool_of_val (Vint n) (negb (Int.eq n Int.zero)).
 
 (** Arithmetic operations *)
 
@@ -128,30 +219,66 @@ Definition absf (v: val) : val :=
   | _ => Vundef
   end.
 
+Definition negfs (v: val) : val :=
+  match v with
+  | Vsingle f => Vsingle (Float32.neg f)
+  | _ => Vundef
+  end.
+
+Definition absfs (v: val) : val :=
+  match v with
+  | Vsingle f => Vsingle (Float32.abs f)
+  | _ => Vundef
+  end.
+
 Definition maketotal (ov: option val) : val :=
   match ov with Some v => v | None => Vundef end.
 
 Definition intoffloat (v: val) : option val :=
   match v with
-  | Vfloat f => option_map Vint (Float.intoffloat f)
+  | Vfloat f => option_map Vint (Float.to_int f)
   | _ => None
   end.
 
 Definition intuoffloat (v: val) : option val :=
   match v with
-  | Vfloat f => option_map Vint (Float.intuoffloat f)
+  | Vfloat f => option_map Vint (Float.to_intu f)
   | _ => None
   end.
 
 Definition floatofint (v: val) : option val :=
   match v with
-  | Vint n => Some (Vfloat (Float.floatofint n))
+  | Vint n => Some (Vfloat (Float.of_int n))
   | _ => None
   end.
 
 Definition floatofintu (v: val) : option val :=
   match v with
-  | Vint n => Some (Vfloat (Float.floatofintu n))
+  | Vint n => Some (Vfloat (Float.of_intu n))
+  | _ => None
+  end.
+
+Definition intofsingle (v: val) : option val :=
+  match v with
+  | Vsingle f => option_map Vint (Float32.to_int f)
+  | _ => None
+  end.
+
+Definition intuofsingle (v: val) : option val :=
+  match v with
+  | Vsingle f => option_map Vint (Float32.to_intu f)
+  | _ => None
+  end.
+
+Definition singleofint (v: val) : option val :=
+  match v with
+  | Vint n => Some (Vsingle (Float32.of_int n))
+  | _ => None
+  end.
+
+Definition singleofintu (v: val) : option val :=
+  match v with
+  | Vint n => Some (Vsingle (Float32.of_intu n))
   | _ => None
   end.
 
@@ -197,24 +324,31 @@ Definition sign_ext (nbits: Z) (v: val) : val :=
 
 Definition singleoffloat (v: val) : val :=
   match v with
-  | Vfloat f => Vfloat(Float.singleoffloat f)
+  | Vfloat f => Vsingle (Float.to_single f)
+  | _ => Vundef
+  end.
+
+Definition floatofsingle (v: val) : val :=
+  match v with
+  | Vsingle f => Vfloat (Float.of_single f)
   | _ => Vundef
   end.
 
 Definition add (v1 v2: val): val :=
   match v1, v2 with
   | Vint n1, Vint n2 => Vint(Int.add n1 n2)
-  | Vptr b1 ofs1, Vint n2 => Vptr b1 (Int.add ofs1 n2)
-  | Vint n1, Vptr b2 ofs2 => Vptr b2 (Int.add ofs2 n1)
+  | Vptr b1 ofs1, Vint n2 => if Archi.ptr64 then Vundef else Vptr b1 (Ptrofs.add ofs1 (Ptrofs.of_int n2))
+  | Vint n1, Vptr b2 ofs2 => if Archi.ptr64 then Vundef else Vptr b2 (Ptrofs.add ofs2 (Ptrofs.of_int n1))
   | _, _ => Vundef
   end.
 
 Definition sub (v1 v2: val): val :=
   match v1, v2 with
   | Vint n1, Vint n2 => Vint(Int.sub n1 n2)
-  | Vptr b1 ofs1, Vint n2 => Vptr b1 (Int.sub ofs1 n2)
+  | Vptr b1 ofs1, Vint n2 => if Archi.ptr64 then Vundef else Vptr b1 (Ptrofs.sub ofs1 (Ptrofs.of_int n2))
   | Vptr b1 ofs1, Vptr b2 ofs2 =>
-      if eq_block b1 b2 then Vint(Int.sub ofs1 ofs2) else Vundef
+      if Archi.ptr64 then Vundef else
+      if eq_block b1 b2 then Vint(Ptrofs.to_int (Ptrofs.sub ofs1 ofs2)) else Vundef
   | _, _ => Vundef
   end.
 
@@ -351,6 +485,12 @@ Definition shru (v1 v2: val): val :=
   | _, _ => Vundef
   end.
 
+Definition rol (v1 v2: val): val :=
+  match v1, v2 with
+  | Vint n1, Vint n2 => Vint(Int.rol n1 n2)
+  | _, _ => Vundef
+  end.
+
 Definition rolm (v: val) (amount mask: int): val :=
   match v with
   | Vint n => Vint(Int.rolm n amount mask)
@@ -359,10 +499,7 @@ Definition rolm (v: val) (amount mask: int): val :=
 
 Definition ror (v1 v2: val): val :=
   match v1, v2 with
-  | Vint n1, Vint n2 =>
-     if Int.ltu n2 Int.iwordsize
-     then Vint(Int.ror n1 n2)
-     else Vundef
+  | Vint n1, Vint n2 => Vint(Int.ror n1 n2)
   | _, _ => Vundef
   end.
 
@@ -393,6 +530,30 @@ Definition divf (v1 v2: val): val :=
 Definition floatofwords (v1 v2: val) : val :=
   match v1, v2 with
   | Vint n1, Vint n2 => Vfloat (Float.from_words n1 n2)
+  | _, _ => Vundef
+  end.
+
+Definition addfs (v1 v2: val): val :=
+  match v1, v2 with
+  | Vsingle f1, Vsingle f2 => Vsingle(Float32.add f1 f2)
+  | _, _ => Vundef
+  end.
+
+Definition subfs (v1 v2: val): val :=
+  match v1, v2 with
+  | Vsingle f1, Vsingle f2 => Vsingle(Float32.sub f1 f2)
+  | _, _ => Vundef
+  end.
+
+Definition mulfs (v1 v2: val): val :=
+  match v1, v2 with
+  | Vsingle f1, Vsingle f2 => Vsingle(Float32.mul f1 f2)
+  | _, _ => Vundef
+  end.
+
+Definition divfs (v1 v2: val): val :=
+  match v1, v2 with
+  | Vsingle f1, Vsingle f2 => Vsingle(Float32.div f1 f2)
   | _, _ => Vundef
   end.
 
@@ -442,49 +603,68 @@ Definition longofintu (v: val) : val :=
 
 Definition longoffloat (v: val) : option val :=
   match v with
-  | Vfloat f => option_map Vlong (Float.longoffloat f)
+  | Vfloat f => option_map Vlong (Float.to_long f)
   | _ => None
   end.
 
 Definition longuoffloat (v: val) : option val :=
   match v with
-  | Vfloat f => option_map Vlong (Float.longuoffloat f)
+  | Vfloat f => option_map Vlong (Float.to_longu f)
+  | _ => None
+  end.
+
+Definition longofsingle (v: val) : option val :=
+  match v with
+  | Vsingle f => option_map Vlong (Float32.to_long f)
+  | _ => None
+  end.
+
+Definition longuofsingle (v: val) : option val :=
+  match v with
+  | Vsingle f => option_map Vlong (Float32.to_longu f)
   | _ => None
   end.
 
 Definition floatoflong (v: val) : option val :=
   match v with
-  | Vlong n => Some (Vfloat (Float.floatoflong n))
+  | Vlong n => Some (Vfloat (Float.of_long n))
   | _ => None
   end.
 
 Definition floatoflongu (v: val) : option val :=
   match v with
-  | Vlong n => Some (Vfloat (Float.floatoflongu n))
+  | Vlong n => Some (Vfloat (Float.of_longu n))
   | _ => None
   end.
 
 Definition singleoflong (v: val) : option val :=
   match v with
-  | Vlong n => Some (Vfloat (Float.singleoflong n))
+  | Vlong n => Some (Vsingle (Float32.of_long n))
   | _ => None
   end.
 
 Definition singleoflongu (v: val) : option val :=
   match v with
-  | Vlong n => Some (Vfloat (Float.singleoflongu n))
+  | Vlong n => Some (Vsingle (Float32.of_longu n))
   | _ => None
   end.
 
 Definition addl (v1 v2: val): val :=
   match v1, v2 with
   | Vlong n1, Vlong n2 => Vlong(Int64.add n1 n2)
+  | Vptr b1 ofs1, Vlong n2 => if Archi.ptr64 then Vptr b1 (Ptrofs.add ofs1 (Ptrofs.of_int64 n2)) else Vundef
+  | Vlong n1, Vptr b2 ofs2 => if Archi.ptr64 then Vptr b2 (Ptrofs.add ofs2 (Ptrofs.of_int64 n1)) else Vundef
   | _, _ => Vundef
   end.
 
 Definition subl (v1 v2: val): val :=
   match v1, v2 with
   | Vlong n1, Vlong n2 => Vlong(Int64.sub n1 n2)
+  | Vptr b1 ofs1, Vlong n2 =>
+      if Archi.ptr64 then Vptr b1 (Ptrofs.sub ofs1 (Ptrofs.of_int64 n2)) else Vundef
+  | Vptr b1 ofs1, Vptr b2 ofs2 =>
+      if negb Archi.ptr64 then Vundef else
+      if eq_block b1 b2 then Vlong(Ptrofs.to_int64 (Ptrofs.sub ofs1 ofs2)) else Vundef
   | _, _ => Vundef
   end.
 
@@ -497,6 +677,18 @@ Definition mull (v1 v2: val): val :=
 Definition mull' (v1 v2: val): val :=
   match v1, v2 with
   | Vint n1, Vint n2 => Vlong(Int64.mul' n1 n2)
+  | _, _ => Vundef
+  end.
+
+Definition mullhs (v1 v2: val): val :=
+  match v1, v2 with
+  | Vlong n1, Vlong n2 => Vlong(Int64.mulhs n1 n2)
+  | _, _ => Vundef
+  end.
+
+Definition mullhu (v1 v2: val): val :=
+  match v1, v2 with
+  | Vlong n1, Vlong n2 => Vlong(Int64.mulhu n1 n2)
   | _, _ => Vundef
   end.
 
@@ -532,6 +724,24 @@ Definition modlu (v1 v2: val): option val :=
   | Vlong n1, Vlong n2 =>
       if Int64.eq n2 Int64.zero then None else Some(Vlong(Int64.modu n1 n2))
   | _, _ => None
+  end.
+
+Definition addl_carry (v1 v2 cin: val): val :=
+  match v1, v2, cin with
+  | Vlong n1, Vlong n2, Vlong c => Vlong(Int64.add_carry n1 n2 c)
+  | _, _, _ => Vundef
+  end.
+
+Definition subl_overflow (v1 v2: val) : val :=
+  match v1, v2 with
+  | Vlong n1, Vlong n2 => Vint (Int.repr (Int64.unsigned (Int64.sub_overflow n1 n2 Int64.zero)))
+  | _, _ => Vundef
+  end.
+
+Definition negativel (v: val) : val :=
+  match v with
+  | Vlong n => Vint (Int.repr (Int64.unsigned (Int64.negative n)))
+  | _ => Vundef
   end.
 
 Definition andl (v1 v2: val): val :=
@@ -579,6 +789,54 @@ Definition shrlu (v1 v2: val): val :=
   | _, _ => Vundef
   end.
 
+Definition shrxl (v1 v2: val): option val :=
+  match v1, v2 with
+  | Vlong n1, Vint n2 =>
+     if Int.ltu n2 (Int.repr 63)
+     then Some(Vlong(Int64.shrx' n1 n2))
+     else None
+  | _, _ => None
+  end.
+
+Definition shrl_carry (v1 v2: val): val :=
+  match v1, v2 with
+  | Vlong n1, Vint n2 =>
+     if Int.ltu n2 Int64.iwordsize'
+     then Vlong(Int64.shr_carry' n1 n2)
+     else Vundef
+  | _, _ => Vundef
+  end.
+
+Definition roll (v1 v2: val): val :=
+  match v1, v2 with
+  | Vlong n1, Vint n2 => Vlong(Int64.rol n1 (Int64.repr (Int.unsigned n2)))
+  | _, _ => Vundef
+  end.
+
+Definition rorl (v1 v2: val): val :=
+  match v1, v2 with
+  | Vlong n1, Vint n2 => Vlong(Int64.ror n1 (Int64.repr (Int.unsigned n2)))
+  | _, _ => Vundef
+  end.
+
+Definition rolml (v: val) (amount: int) (mask: int64): val :=
+  match v with
+  | Vlong n => Vlong(Int64.rolm n (Int64.repr (Int.unsigned amount)) mask)
+  | _ => Vundef
+  end.
+
+Definition zero_ext_l (nbits: Z) (v: val) : val :=
+  match v with
+  | Vlong n => Vlong(Int64.zero_ext nbits n)
+  | _ => Vundef
+  end.
+
+Definition sign_ext_l (nbits: Z) (v: val) : val :=
+  match v with
+  | Vlong n => Vlong(Int64.sign_ext nbits n)
+  | _ => Vundef
+  end.
+
 (** Comparisons *)
 
 Section COMPARISONS.
@@ -604,26 +862,39 @@ Definition cmpu_bool (c: comparison) (v1 v2: val): option bool :=
   | Vint n1, Vint n2 =>
       Some (Int.cmpu c n1 n2)
   | Vint n1, Vptr b2 ofs2 =>
-      if Int.eq n1 Int.zero then cmp_different_blocks c else None
+      if Archi.ptr64 then None else
+      if Int.eq n1 Int.zero && weak_valid_ptr b2 (Ptrofs.unsigned ofs2)
+      then cmp_different_blocks c
+      else None
   | Vptr b1 ofs1, Vptr b2 ofs2 =>
+      if Archi.ptr64 then None else
       if eq_block b1 b2 then
-        if weak_valid_ptr b1 (Int.unsigned ofs1)
-           && weak_valid_ptr b2 (Int.unsigned ofs2)
-        then Some (Int.cmpu c ofs1 ofs2)
+        if weak_valid_ptr b1 (Ptrofs.unsigned ofs1)
+           && weak_valid_ptr b2 (Ptrofs.unsigned ofs2)
+        then Some (Ptrofs.cmpu c ofs1 ofs2)
         else None
       else
-        if valid_ptr b1 (Int.unsigned ofs1)
-           && valid_ptr b2 (Int.unsigned ofs2)
+        if valid_ptr b1 (Ptrofs.unsigned ofs1)
+           && valid_ptr b2 (Ptrofs.unsigned ofs2)
         then cmp_different_blocks c
         else None
   | Vptr b1 ofs1, Vint n2 =>
-      if Int.eq n2 Int.zero then cmp_different_blocks c else None
+      if Archi.ptr64 then None else
+      if Int.eq n2 Int.zero && weak_valid_ptr b1 (Ptrofs.unsigned ofs1)
+      then cmp_different_blocks c
+      else None
   | _, _ => None
   end.
 
 Definition cmpf_bool (c: comparison) (v1 v2: val): option bool :=
   match v1, v2 with
   | Vfloat f1, Vfloat f2 => Some (Float.cmp c f1 f2)
+  | _, _ => None
+  end.
+
+Definition cmpfs_bool (c: comparison) (v1 v2: val): option bool :=
+  match v1, v2 with
+  | Vsingle f1, Vsingle f2 => Some (Float32.cmp c f1 f2)
   | _, _ => None
   end.
 
@@ -636,6 +907,28 @@ Definition cmpl_bool (c: comparison) (v1 v2: val): option bool :=
 Definition cmplu_bool (c: comparison) (v1 v2: val): option bool :=
   match v1, v2 with
   | Vlong n1, Vlong n2 => Some (Int64.cmpu c n1 n2)
+  | Vlong n1, Vptr b2 ofs2 =>
+      if negb Archi.ptr64 then None else
+      if Int64.eq n1 Int64.zero && weak_valid_ptr b2 (Ptrofs.unsigned ofs2)
+      then cmp_different_blocks c
+      else None
+  | Vptr b1 ofs1, Vptr b2 ofs2 =>
+      if negb Archi.ptr64 then None else
+      if eq_block b1 b2 then
+        if weak_valid_ptr b1 (Ptrofs.unsigned ofs1)
+           && weak_valid_ptr b2 (Ptrofs.unsigned ofs2)
+        then Some (Ptrofs.cmpu c ofs1 ofs2)
+        else None
+      else
+        if valid_ptr b1 (Ptrofs.unsigned ofs1)
+           && valid_ptr b2 (Ptrofs.unsigned ofs2)
+        then cmp_different_blocks c
+        else None
+  | Vptr b1 ofs1, Vlong n2 =>
+      if negb Archi.ptr64 then None else
+      if Int64.eq n2 Int64.zero && weak_valid_ptr b1 (Ptrofs.unsigned ofs1)
+      then cmp_different_blocks c
+      else None
   | _, _ => None
   end.
 
@@ -651,6 +944,9 @@ Definition cmpu (c: comparison) (v1 v2: val): val :=
 Definition cmpf (c: comparison) (v1 v2: val): val :=
   of_optbool (cmpf_bool c v1 v2).
 
+Definition cmpfs (c: comparison) (v1 v2: val): val :=
+  of_optbool (cmpfs_bool c v1 v2).
+
 Definition cmpl (c: comparison) (v1 v2: val): option val :=
   option_map of_bool (cmpl_bool c v1 v2).
 
@@ -664,6 +960,68 @@ Definition maskzero_bool (v: val) (mask: int): option bool :=
   end.
 
 End COMPARISONS.
+
+(** Add the given offset to the given pointer. *)
+
+Definition offset_ptr (v: val) (delta: ptrofs) : val :=
+  match v with
+  | Vptr b ofs => Vptr b (Ptrofs.add ofs delta)
+  | _ => Vundef
+  end.
+
+(** Normalize a value to the given type, turning it into Vundef if it does not
+    match the type. *)
+
+Definition normalize (v: val) (ty: typ) : val :=
+  match v, ty with
+  | Vundef, _ => Vundef
+  | Vint _, Tint => v
+  | Vlong _, Tlong => v
+  | Vfloat _, Tfloat => v
+  | Vsingle _, Tsingle => v
+  | Vptr _ _, (Tint | Tany32) => if Archi.ptr64 then Vundef else v
+  | Vptr _ _, Tlong => if Archi.ptr64 then v else Vundef
+  | (Vint _ | Vsingle _), Tany32 => v
+  | (Vint _ | Vsingle _ | Vlong _ | Vfloat _ | Vptr _ _), Tany64 => v
+  | Vvec t1 _, Tvec t2 => if Archi.vec_typ_eq t1 t2 then v else Vundef
+  | _, _ => Vundef
+  end.
+
+Lemma normalize_type:
+  forall v ty, has_type (normalize v ty) ty.
+Proof.
+  intros; destruct v; simpl.
+- auto.
+- destruct ty; exact I.
+- destruct ty; exact I.
+- destruct ty; exact I.
+- destruct ty; exact I.
+- unfold has_type; destruct ty, Archi.ptr64; auto.
+- unfold has_type; destruct ty; auto.
+  destruct (Archi.vec_typ_eq t v0); auto.
+Qed.
+
+Lemma normalize_idem:
+  forall v ty, has_type v ty -> normalize v ty = v.
+Proof.
+  unfold has_type, normalize; intros. destruct v.
+- auto.
+- destruct ty; intuition auto.
+- destruct ty; intuition auto.
+- destruct ty; intuition auto.
+- destruct ty; intuition auto.
+- destruct ty, Archi.ptr64; intuition congruence.
+- destruct ty; elim H.
+  destruct (Archi.vec_typ_eq t t); congruence.
+Qed.
+
+(** Select between two values based on the result of a comparison. *)
+
+Definition select (cmp: option bool) (v1 v2: val) (ty: typ) :=
+  match cmp with
+  | Some b => normalize (if b then v1 else v2) ty
+  | None => Vundef
+  end.
 
 (** [load_result] reflects the effect of storing a value with a given
   memory chunk, then reading it back with the same chunk.  Depending
@@ -681,25 +1039,45 @@ Definition load_result (chunk: memory_chunk) (v: val) :=
   | Mint16signed, Vint n => Vint (Int.sign_ext 16 n)
   | Mint16unsigned, Vint n => Vint (Int.zero_ext 16 n)
   | Mint32, Vint n => Vint n
-  | Mint32, Vptr b ofs => Vptr b ofs
+  | Mint32, Vptr b ofs => if Archi.ptr64 then Vundef else Vptr b ofs
   | Mint64, Vlong n => Vlong n
-  | Mint128, V128 n => V128 n
-  | Mfloat32, Vfloat f => Vfloat(Float.singleoffloat f)
+  | Mint64, Vptr b ofs => if Archi.ptr64 then Vptr b ofs else Vundef
+  | Mfloat32, Vsingle f => Vsingle f
   | Mfloat64, Vfloat f => Vfloat f
+  | Many32, (Vint _ | Vsingle _) => v
+  | Many32, Vptr _ _ => if Archi.ptr64 then Vundef else v
+  | Many64, (Vint _ | Vsingle _ | Vlong _ | Vfloat _ | Vptr _ _) => v
+  | Mvec t, Vvec t' v => if Archi.vec_typ_eq t t' then Vvec t' v else Vundef
   | _, _ => Vundef
   end.
+
+Lemma load_result_rettype:
+  forall chunk v, has_rettype (load_result chunk v) (rettype_of_chunk chunk).
+Proof.
+  intros. unfold has_rettype; destruct chunk; destruct v; simpl; auto.
+- rewrite Int.sign_ext_idem by omega; auto.
+- rewrite Int.zero_ext_idem by omega; auto.
+- rewrite Int.sign_ext_idem by omega; auto.
+- rewrite Int.zero_ext_idem by omega; auto.
+- destruct Archi.ptr64 eqn:SF; simpl; auto.
+- destruct Archi.ptr64 eqn:SF; simpl; auto.
+- destruct Archi.ptr64 eqn:SF; simpl; auto.
+- destruct (Archi.vec_typ_eq v0 t); simpl; auto.
+Qed.
 
 Lemma load_result_type:
   forall chunk v, has_type (load_result chunk v) (type_of_chunk chunk).
 Proof.
-  intros. destruct chunk; destruct v; simpl; auto. apply Float.singleoffloat_is_single.
+  intros. rewrite <- proj_rettype_of_chunk. apply has_proj_rettype.
+  apply load_result_rettype.
 Qed.
 
 Lemma load_result_same:
   forall v ty, has_type v ty -> load_result (chunk_of_type ty) v = v.
 Proof.
-  unfold has_type; intros. destruct v; destruct ty; try contradiction; auto.
-  simpl. rewrite Float.singleoffloat_of_single; auto. 
+  unfold has_type, load_result; intros.
+  destruct v; destruct ty; destruct Archi.ptr64; try contradiction; try discriminate; simpl; auto;
+  revert H; destruct (Archi.vec_typ_eq v0 t); auto; intros; elim n; rewrite H; reflexivity. 
 Qed.
 
 (** Theorems on arithmetic operations. *)
@@ -707,14 +1085,14 @@ Qed.
 Theorem cast8unsigned_and:
   forall x, zero_ext 8 x = and x (Vint(Int.repr 255)).
 Proof.
-  destruct x; simpl; auto. decEq. 
-  change 255 with (two_p 8 - 1). apply Int.zero_ext_and. omega. 
+  destruct x; simpl; auto. decEq.
+  change 255 with (two_p 8 - 1). apply Int.zero_ext_and. omega.
 Qed.
 
 Theorem cast16unsigned_and:
   forall x, zero_ext 16 x = and x (Vint(Int.repr 65535)).
 Proof.
-  destruct x; simpl; auto. decEq. 
+  destruct x; simpl; auto. decEq.
   change 65535 with (two_p 16 - 1). apply Int.zero_ext_and. omega.
 Qed.
 
@@ -727,7 +1105,7 @@ Qed.
 Theorem bool_of_val_of_optbool:
   forall ob b, bool_of_val (of_optbool ob) b -> ob = Some b.
 Proof.
-  intros. destruct ob; simpl in H. 
+  intros. destruct ob; simpl in H.
   destruct b0; simpl in H; inv H; auto.
   inv H.
 Qed.
@@ -759,7 +1137,7 @@ Qed.
 Theorem notbool_idem3:
   forall x, notbool(notbool(notbool x)) = notbool x.
 Proof.
-  destruct x; simpl; auto. 
+  destruct x; simpl; auto.
   case (Int.eq i Int.zero); reflexivity.
 Qed.
 
@@ -777,13 +1155,15 @@ Qed.
 
 Theorem add_assoc: forall x y z, add (add x y) z = add x (add y z).
 Proof.
-  destruct x; destruct y; destruct z; simpl; auto.
-  rewrite Int.add_assoc; auto.
-  rewrite Int.add_assoc; auto.
-  decEq. decEq. apply Int.add_commut.
-  decEq. rewrite Int.add_commut. rewrite <- Int.add_assoc. 
-  decEq. apply Int.add_commut.
-  decEq. rewrite Int.add_assoc. auto.
+  unfold add; intros; destruct Archi.ptr64 eqn:SF, x, y, z; simpl; auto.
+- rewrite Int.add_assoc; auto.
+- rewrite Int.add_assoc; auto.
+- rewrite ! Ptrofs.add_assoc. f_equal. f_equal.
+  rewrite Ptrofs.add_commut. auto with ptrofs.
+- rewrite ! Ptrofs.add_assoc. f_equal. f_equal.
+  apply Ptrofs.add_commut.
+- rewrite ! Ptrofs.add_assoc. f_equal. f_equal.
+  symmetry. auto with ptrofs.
 Qed.
 
 Theorem add_permut: forall x y z, add x (add y z) = add y (add x z).
@@ -794,8 +1174,8 @@ Qed.
 Theorem add_permut_4:
   forall x y z t, add (add x y) (add z t) = add (add x z) (add y t).
 Proof.
-  intros. rewrite add_permut. rewrite add_assoc. 
-  rewrite add_permut. symmetry. apply add_assoc. 
+  intros. rewrite add_permut. rewrite add_assoc.
+  rewrite add_permut. symmetry. apply add_assoc.
 Qed.
 
 Theorem neg_zero: neg Vzero = Vzero.
@@ -805,47 +1185,51 @@ Qed.
 
 Theorem neg_add_distr: forall x y, neg(add x y) = add (neg x) (neg y).
 Proof.
-  destruct x; destruct y; simpl; auto. decEq. apply Int.neg_add_distr.
+  unfold neg, add; intros; destruct Archi.ptr64 eqn:SF, x, y; simpl; auto;
+  rewrite Int.neg_add_distr; auto.
 Qed.
 
 Theorem sub_zero_r: forall x, sub Vzero x = neg x.
 Proof.
-  destruct x; simpl; auto. 
+  destruct x; simpl; auto.
 Qed.
 
 Theorem sub_add_opp: forall x y, sub x (Vint y) = add x (Vint (Int.neg y)).
 Proof.
-  destruct x; intro y; simpl; auto; rewrite Int.sub_add_opp; auto.
+  unfold sub, add; intros; destruct Archi.ptr64 eqn:SF, x; auto.
+- rewrite Int.sub_add_opp; auto.
+- rewrite Int.sub_add_opp; auto.
+- rewrite Ptrofs.sub_add_opp. f_equal. f_equal. symmetry. auto with ptrofs.
 Qed.
 
 Theorem sub_opp_add: forall x y, sub x (Vint (Int.neg y)) = add x (Vint y).
 Proof.
-  intros. unfold sub, add.
-  destruct x; auto; rewrite Int.sub_add_opp; rewrite Int.neg_involutive; auto.
+  intros. rewrite sub_add_opp. rewrite Int.neg_involutive. auto.
 Qed.
 
 Theorem sub_add_l:
   forall v1 v2 i, sub (add v1 (Vint i)) v2 = add (sub v1 v2) (Vint i).
 Proof.
-  destruct v1; destruct v2; intros; simpl; auto.
-  rewrite Int.sub_add_l. auto.
-  rewrite Int.sub_add_l. auto.
-  case (eq_block b b0); intro. rewrite Int.sub_add_l. auto. reflexivity.
+  unfold sub, add; intros; destruct Archi.ptr64 eqn:SF, v1, v2; auto.
+- rewrite Int.sub_add_l; auto.
+- rewrite Int.sub_add_l; auto.
+- rewrite Ptrofs.sub_add_l; auto.
+- destruct (eq_block b b0); auto.
+  f_equal. rewrite Ptrofs.sub_add_l. auto with ptrofs.
 Qed.
 
 Theorem sub_add_r:
   forall v1 v2 i, sub v1 (add v2 (Vint i)) = add (sub v1 v2) (Vint (Int.neg i)).
 Proof.
-  destruct v1; destruct v2; intros; simpl; auto.
-  rewrite Int.sub_add_r. auto.
-  repeat rewrite Int.sub_add_opp. decEq. 
-  repeat rewrite Int.add_assoc. decEq. apply Int.add_commut.
-  decEq. repeat rewrite Int.sub_add_opp. 
-  rewrite Int.add_assoc. decEq. apply Int.neg_add_distr.
-  case (eq_block b b0); intro. simpl. decEq. 
-  repeat rewrite Int.sub_add_opp. rewrite Int.add_assoc. decEq.
-  apply Int.neg_add_distr.
-  reflexivity.
+  unfold sub, add; intros; destruct Archi.ptr64 eqn:SF, v1, v2; auto.
+- rewrite Int.add_commut. rewrite Int.sub_add_r. auto.
+- rewrite Int.add_commut. rewrite Int.sub_add_r. auto.
+- f_equal. replace (Ptrofs.of_int (Int.add i1 i)) with (Ptrofs.add (Ptrofs.of_int i) (Ptrofs.of_int i1)).
+  rewrite Ptrofs.sub_add_r. f_equal.
+  symmetry. auto with ptrofs.
+  symmetry. rewrite Int.add_commut. auto with ptrofs.
+- destruct (eq_block b b0); auto.
+  f_equal. rewrite Ptrofs.add_commut. rewrite Ptrofs.sub_add_r. auto with ptrofs.
 Qed.
 
 Theorem mul_commut: forall x y, mul x y = mul y x.
@@ -862,16 +1246,15 @@ Qed.
 Theorem mul_add_distr_l:
   forall x y z, mul (add x y) z = add (mul x z) (mul y z).
 Proof.
-  destruct x; destruct y; destruct z; simpl; auto.
-  decEq. apply Int.mul_add_distr_l.
+  unfold mul, add; intros; destruct Archi.ptr64 eqn:SF, x, y, z; simpl; auto;
+  rewrite Int.mul_add_distr_l; auto.
 Qed.
-
 
 Theorem mul_add_distr_r:
   forall x y z, mul x (add y z) = add (mul x y) (mul x z).
 Proof.
-  destruct x; destruct y; destruct z; simpl; auto.
-  decEq. apply Int.mul_add_distr_r.
+  unfold mul, add; intros; destruct Archi.ptr64 eqn:SF, x, y, z; simpl; auto;
+  rewrite Int.mul_add_distr_r; auto.
 Qed.
 
 Theorem mul_pow2:
@@ -882,7 +1265,7 @@ Proof.
   intros; destruct x; simpl; auto.
   change 32 with Int.zwordsize.
   rewrite (Int.is_power2_range _ _ H). decEq. apply Int.mul_pow2. auto.
-Qed.  
+Qed.
 
 Theorem mods_divs:
   forall x y z,
@@ -891,7 +1274,7 @@ Proof.
   intros. destruct x; destruct y; simpl in *; try discriminate.
   destruct (Int.eq i0 Int.zero
         || Int.eq i (Int.repr Int.min_signed) && Int.eq i0 Int.mone); inv H.
-  exists (Vint (Int.divs i i0)); split; auto. 
+  exists (Vint (Int.divs i i0)); split; auto.
   simpl. rewrite Int.mods_divs. auto.
 Qed.
 
@@ -900,10 +1283,32 @@ Theorem modu_divu:
   modu x y = Some z -> exists v, divu x y = Some v /\ z = sub x (mul v y).
 Proof.
   intros. destruct x; destruct y; simpl in *; try discriminate.
-  destruct (Int.eq i0 Int.zero) eqn:?; inv H. 
-  exists (Vint (Int.divu i i0)); split; auto. 
+  destruct (Int.eq i0 Int.zero) eqn:?; inv H.
+  exists (Vint (Int.divu i i0)); split; auto.
   simpl. rewrite Int.modu_divu. auto.
-  generalize (Int.eq_spec i0 Int.zero). rewrite Heqb; auto. 
+  generalize (Int.eq_spec i0 Int.zero). rewrite Heqb; auto.
+Qed.
+
+Theorem modls_divls:
+  forall x y z,
+  modls x y = Some z -> exists v, divls x y = Some v /\ z = subl x (mull v y).
+Proof.
+  intros. destruct x; destruct y; simpl in *; try discriminate.
+  destruct (Int64.eq i0 Int64.zero
+        || Int64.eq i (Int64.repr Int64.min_signed) && Int64.eq i0 Int64.mone); inv H.
+  exists (Vlong (Int64.divs i i0)); split; auto.
+  simpl. rewrite Int64.mods_divs. auto.
+Qed.
+
+Theorem modlu_divlu:
+  forall x y z,
+  modlu x y = Some z -> exists v, divlu x y = Some v /\ z = subl x (mull v y).
+Proof.
+  intros. destruct x; destruct y; simpl in *; try discriminate.
+  destruct (Int64.eq i0 Int64.zero) eqn:?; inv H.
+  exists (Vlong (Int64.divu i i0)); split; auto.
+  simpl. rewrite Int64.modu_divu. auto.
+  generalize (Int64.eq_spec i0 Int64.zero). rewrite Heqb; auto.
 Qed.
 
 Theorem divs_pow2:
@@ -918,6 +1323,16 @@ Proof.
   simpl. rewrite H0. decEq. decEq. symmetry. apply Int.divs_pow2. auto.
 Qed.
 
+Theorem divs_one:
+  forall s , divs (Vint s) (Vint Int.one) = Some (Vint s).
+Proof.
+   intros.
+   unfold divs. rewrite Int.eq_false; try discriminate.
+   simpl. rewrite (Int.eq_false Int.one Int.mone); try discriminate.
+   rewrite andb_false_intro2; auto. f_equal. f_equal.
+   rewrite Int.divs_one; auto. replace Int.zwordsize with 32; auto. omega.
+Qed.
+
 Theorem divu_pow2:
   forall x n logn y,
   Int.is_power2 n = Some logn ->
@@ -925,10 +1340,17 @@ Theorem divu_pow2:
   shru x (Vint logn) = y.
 Proof.
   intros; destruct x; simpl in H0; inv H0.
-  destruct (Int.eq n Int.zero); inv H2. 
-  simpl. 
+  destruct (Int.eq n Int.zero); inv H2.
+  simpl.
   rewrite (Int.is_power2_range _ _ H).
   decEq. symmetry. apply Int.divu_pow2. auto.
+Qed.
+
+Theorem divu_one:
+  forall s, divu (Vint s) (Vint Int.one) = Some (Vint s).
+Proof.
+  intros. simpl. rewrite Int.eq_false; try discriminate.
+  f_equal. f_equal. apply Int.divu_one.
 Qed.
 
 Theorem modu_pow2:
@@ -938,7 +1360,7 @@ Theorem modu_pow2:
   and x (Vint (Int.sub n Int.one)) = y.
 Proof.
   intros; destruct x; simpl in H0; inv H0.
-  destruct (Int.eq n Int.zero); inv H2. 
+  destruct (Int.eq n Int.zero); inv H2.
   simpl. decEq. symmetry. eapply Int.modu_and; eauto.
 Qed.
 
@@ -977,12 +1399,12 @@ Qed.
 
 Theorem not_xor: forall x, notint x = xor x (Vint Int.mone).
 Proof.
-  destruct x; simpl; auto. 
+  destruct x; simpl; auto.
 Qed.
 
 Theorem shl_mul: forall x y, mul x (shl Vone y) = shl x y.
 Proof.
-  destruct x; destruct y; simpl; auto. 
+  destruct x; destruct y; simpl; auto.
   case (Int.ltu i0 Int.iwordsize); auto.
   decEq. symmetry. apply Int.shl_mul.
 Qed.
@@ -996,6 +1418,16 @@ Proof.
   rewrite H. decEq. apply Int.shl_rolm. exact H.
 Qed.
 
+Theorem shll_rolml:
+  forall x n,
+  Int.ltu n Int64.iwordsize' = true ->
+  shll x (Vint n) = rolml x n (Int64.shl Int64.mone (Int64.repr (Int.unsigned n))).
+Proof.
+  intros. destruct x; auto. simpl. rewrite H. rewrite <- Int64.shl_rolm. unfold Int64.shl.
+  rewrite Int64.int_unsigned_repr. constructor. unfold Int64.ltu. rewrite Int64.int_unsigned_repr.
+  apply H.
+Qed.
+
 Theorem shru_rolm:
   forall x n,
   Int.ltu n Int.iwordsize = true ->
@@ -1005,16 +1437,27 @@ Proof.
   rewrite H. decEq. apply Int.shru_rolm. exact H.
 Qed.
 
+Theorem shrlu_rolml:
+  forall x n,
+    Int.ltu n Int64.iwordsize' = true ->
+    shrlu x (Vint n) = rolml x (Int.sub Int64.iwordsize' n) (Int64.shru Int64.mone (Int64.repr (Int.unsigned n))).
+Proof.
+  intros. destruct x; auto. simpl. rewrite H.
+  rewrite Int64.int_sub_ltu by apply H. rewrite Int64.repr_unsigned. rewrite <- Int64.shru_rolm. unfold Int64.shru'.  unfold Int64.shru.
+  rewrite Int64.unsigned_repr. reflexivity. apply Int64.int_unsigned_range.
+  unfold Int64.ltu. rewrite Int64.int_unsigned_repr. auto.
+Qed.
+
 Theorem shrx_carry:
   forall x y z,
   shrx x y = Some z ->
   add (shr x y) (shr_carry x y) = z.
 Proof.
-  intros. destruct x; destruct y; simpl in H; inv H. 
+  intros. destruct x; destruct y; simpl in H; inv H.
   destruct (Int.ltu i0 (Int.repr 31)) eqn:?; inv H1.
   exploit Int.ltu_inv; eauto. change (Int.unsigned (Int.repr 31)) with 31. intros.
-  assert (Int.ltu i0 Int.iwordsize = true). 
-    unfold Int.ltu. apply zlt_true. change (Int.unsigned Int.iwordsize) with 32. omega. 
+  assert (Int.ltu i0 Int.iwordsize = true).
+    unfold Int.ltu. apply zlt_true. change (Int.unsigned Int.iwordsize) with 32. omega.
   simpl. rewrite H0. simpl. decEq. rewrite Int.shrx_carry; auto.
 Qed.
 
@@ -1025,13 +1468,39 @@ Theorem shrx_shr:
     x = Vint p /\ y = Vint q /\
     z = shr (if Int.lt p Int.zero then add x (Vint (Int.sub (Int.shl Int.one q) Int.one)) else x) (Vint q).
 Proof.
-  intros. destruct x; destruct y; simpl in H; inv H. 
+  intros. destruct x; destruct y; simpl in H; inv H.
   destruct (Int.ltu i0 (Int.repr 31)) eqn:?; inv H1.
   exploit Int.ltu_inv; eauto. change (Int.unsigned (Int.repr 31)) with 31. intros.
-  assert (Int.ltu i0 Int.iwordsize = true). 
-    unfold Int.ltu. apply zlt_true. change (Int.unsigned Int.iwordsize) with 32. omega. 
-  exists i; exists i0; intuition. 
+  assert (Int.ltu i0 Int.iwordsize = true).
+    unfold Int.ltu. apply zlt_true. change (Int.unsigned Int.iwordsize) with 32. omega.
+  exists i; exists i0; intuition.
   rewrite Int.shrx_shr; auto. destruct (Int.lt i Int.zero); simpl; rewrite H0; auto.
+Qed.
+
+Theorem shrx_shr_2:
+  forall n x z,
+  shrx x (Vint n) = Some z ->
+  z = (if Int.eq n Int.zero then x else
+         shr (add x (shru (shr x (Vint (Int.repr 31)))
+                    (Vint (Int.sub (Int.repr 32) n))))
+             (Vint n)).
+Proof.
+  intros. destruct x; simpl in H; try discriminate.
+  destruct (Int.ltu n (Int.repr 31)) eqn:LT; inv H.
+  exploit Int.ltu_inv; eauto. change (Int.unsigned (Int.repr 31)) with 31; intros LT'.
+  predSpec Int.eq Int.eq_spec n Int.zero.
+- subst n. unfold Int.shrx. rewrite Int.shl_zero. unfold Int.divs. change (Int.signed Int.one) with 1.
+  rewrite Z.quot_1_r. rewrite Int.repr_signed; auto.
+- simpl. change (Int.ltu (Int.repr 31) Int.iwordsize) with true. simpl.
+  replace (Int.ltu (Int.sub (Int.repr 32) n) Int.iwordsize) with true. simpl.
+  replace (Int.ltu n Int.iwordsize) with true.
+  f_equal; apply Int.shrx_shr_2; assumption.
+  symmetry; apply zlt_true. change (Int.unsigned n < 32); omega.
+  symmetry; apply zlt_true. unfold Int.sub. change (Int.unsigned (Int.repr 32)) with 32.
+  assert (Int.unsigned n <> 0). { red; intros; elim H. rewrite <- (Int.repr_unsigned n), H0. auto. }
+  rewrite Int.unsigned_repr.
+  change (Int.unsigned Int.iwordsize) with 32; omega.
+  assert (32 < Int.max_unsigned) by reflexivity. omega.
 Qed.
 
 Theorem or_rolm:
@@ -1049,7 +1518,7 @@ Theorem rolm_rolm:
            (Int.and (Int.rol m1 n2) m2).
 Proof.
   intros; destruct x; simpl; auto.
-  decEq. 
+  decEq.
   apply Int.rolm_rolm. apply int_wordsize_divides_modulus.
 Qed.
 
@@ -1058,6 +1527,239 @@ Theorem rolm_zero:
   rolm x Int.zero m = and x (Vint m).
 Proof.
   intros; destruct x; simpl; auto. decEq. apply Int.rolm_zero.
+Qed.
+
+Theorem addl_commut: forall x y, addl x y = addl y x.
+Proof.
+  destruct x; destruct y; simpl; auto.
+  decEq. apply Int64.add_commut.
+Qed.
+
+Theorem addl_assoc: forall x y z, addl (addl x y) z = addl x (addl y z).
+Proof.
+  unfold addl; intros; destruct Archi.ptr64 eqn:SF, x, y, z; simpl; auto.
+- rewrite Int64.add_assoc; auto.
+- rewrite ! Ptrofs.add_assoc. f_equal. f_equal.
+  rewrite Ptrofs.add_commut. auto with ptrofs.
+- rewrite ! Ptrofs.add_assoc. f_equal. f_equal.
+  apply Ptrofs.add_commut.
+- rewrite ! Ptrofs.add_assoc. f_equal. f_equal.
+  symmetry. auto with ptrofs.
+- rewrite Int64.add_assoc; auto.
+Qed.
+
+Theorem addl_permut: forall x y z, addl x (addl y z) = addl y (addl x z).
+Proof.
+  intros. rewrite (addl_commut y z). rewrite <- addl_assoc. apply addl_commut.
+Qed.
+
+Theorem addl_permut_4:
+  forall x y z t, addl (addl x y) (addl z t) = addl (addl x z) (addl y t).
+Proof.
+  intros. rewrite addl_permut. rewrite addl_assoc.
+  rewrite addl_permut. symmetry. apply addl_assoc.
+Qed.
+
+Theorem negl_addl_distr: forall x y, negl(addl x y) = addl (negl x) (negl y).
+Proof.
+  unfold negl, addl; intros; destruct Archi.ptr64 eqn:SF; destruct x; destruct y; simpl; auto;
+  decEq; apply Int64.neg_add_distr.
+Qed.
+
+Theorem subl_addl_opp: forall x y, subl x (Vlong y) = addl x (Vlong (Int64.neg y)).
+Proof.
+  unfold subl, addl; intros; destruct Archi.ptr64 eqn:SF, x; auto.
+- rewrite Int64.sub_add_opp; auto.
+- rewrite Ptrofs.sub_add_opp. f_equal. f_equal. symmetry. auto with ptrofs.
+- rewrite Int64.sub_add_opp; auto.
+Qed.
+
+Theorem subl_opp_addl: forall x y, subl x (Vlong (Int64.neg y)) = addl x (Vlong y).
+Proof.
+  intros. rewrite subl_addl_opp. rewrite Int64.neg_involutive. auto.
+Qed.
+
+Theorem subl_addl_l:
+  forall v1 v2 i, subl (addl v1 (Vlong i)) v2 = addl (subl v1 v2) (Vlong i).
+Proof.
+  unfold subl, addl; intros; destruct Archi.ptr64 eqn:SF, v1, v2; auto.
+- rewrite Int64.sub_add_l; auto.
+- rewrite Ptrofs.sub_add_l; auto.
+- destruct (eq_block b b0); auto.
+  simpl. f_equal. rewrite Ptrofs.sub_add_l. auto with ptrofs.
+- rewrite Int64.sub_add_l; auto.
+Qed.
+
+Theorem subl_addl_r:
+  forall v1 v2 i, subl v1 (addl v2 (Vlong i)) = addl (subl v1 v2) (Vlong (Int64.neg i)).
+Proof.
+  unfold subl, addl; intros; destruct Archi.ptr64 eqn:SF, v1, v2; auto.
+- rewrite Int64.add_commut. rewrite Int64.sub_add_r. auto.
+- f_equal. replace (Ptrofs.of_int64 (Int64.add i1 i)) with (Ptrofs.add (Ptrofs.of_int64 i) (Ptrofs.of_int64 i1)).
+  rewrite Ptrofs.sub_add_r. f_equal.
+  symmetry. auto with ptrofs.
+  symmetry. rewrite Int64.add_commut. auto with ptrofs.
+- destruct (eq_block b b0); auto.
+  simpl; f_equal. rewrite Ptrofs.add_commut. rewrite Ptrofs.sub_add_r. auto with ptrofs.
+- rewrite Int64.add_commut. rewrite Int64.sub_add_r. auto.
+Qed.
+
+Theorem mull_commut: forall x y, mull x y = mull y x.
+Proof.
+  destruct x; destruct y; simpl; auto. decEq. apply Int64.mul_commut.
+Qed.
+
+Theorem mull_assoc: forall x y z, mull (mull x y) z = mull x (mull y z).
+Proof.
+  destruct x; destruct y; destruct z; simpl; auto.
+  decEq. apply Int64.mul_assoc.
+Qed.
+
+Theorem mull_addl_distr_l:
+  forall x y z, mull (addl x y) z = addl (mull x z) (mull y z).
+Proof.
+  unfold mull, addl; intros; destruct Archi.ptr64 eqn:SF; destruct x; destruct y; destruct z; simpl; auto;
+  decEq; apply Int64.mul_add_distr_l.
+Qed.
+
+Theorem mull_addl_distr_r:
+  forall x y z, mull x (addl y z) = addl (mull x y) (mull x z).
+Proof.
+  unfold mull, addl; intros; destruct Archi.ptr64 eqn:SF; destruct x; destruct y; destruct z; simpl; auto;
+  decEq; apply Int64.mul_add_distr_r.
+Qed.
+
+Theorem andl_commut: forall x y, andl x y = andl y x.
+Proof.
+  destruct x; destruct y; simpl; auto. decEq. apply Int64.and_commut.
+Qed.
+
+Theorem andl_assoc: forall x y z, andl (andl x y) z = andl x (andl y z).
+Proof.
+  destruct x; destruct y; destruct z; simpl; auto.
+  decEq. apply Int64.and_assoc.
+Qed.
+
+Theorem orl_commut: forall x y, orl x y = orl y x.
+Proof.
+  destruct x; destruct y; simpl; auto. decEq. apply Int64.or_commut.
+Qed.
+
+Theorem orl_assoc: forall x y z, orl (orl x y) z = orl x (orl y z).
+Proof.
+  destruct x; destruct y; destruct z; simpl; auto.
+  decEq. apply Int64.or_assoc.
+Qed.
+
+Theorem xorl_commut: forall x y, xorl x y = xorl y x.
+Proof.
+  destruct x; destruct y; simpl; auto. decEq. apply Int64.xor_commut.
+Qed.
+
+Theorem xorl_assoc: forall x y z, xorl (xorl x y) z = xorl x (xorl y z).
+Proof.
+  destruct x; destruct y; destruct z; simpl; auto.
+  decEq. apply Int64.xor_assoc.
+Qed.
+
+Theorem notl_xorl: forall x, notl x = xorl x (Vlong Int64.mone).
+Proof.
+  destruct x; simpl; auto.
+Qed.
+
+Theorem divls_pow2:
+  forall x n logn y,
+  Int64.is_power2' n = Some logn -> Int.ltu logn (Int.repr 63) = true ->
+  divls x (Vlong n) = Some y ->
+  shrxl x (Vint logn) = Some y.
+Proof.
+  intros; destruct x; simpl in H1; inv H1.
+  destruct (Int64.eq n Int64.zero
+         || Int64.eq i (Int64.repr Int64.min_signed) && Int64.eq n Int64.mone); inv H3.
+  simpl. rewrite H0. decEq. decEq.
+  generalize (Int64.is_power2'_correct _ _ H); intro.
+  unfold Int64.shrx'. rewrite Int64.shl'_mul_two_p. rewrite <- H1.
+  rewrite Int64.mul_commut. rewrite Int64.mul_one.
+  rewrite Int64.repr_unsigned. auto.
+Qed.
+
+Theorem divls_one:
+  forall n, divls (Vlong n) (Vlong Int64.one) = Some (Vlong n).
+Proof.
+  intros. unfold divls. rewrite Int64.eq_false; try discriminate.
+  rewrite (Int64.eq_false Int64.one Int64.mone); try discriminate.
+  rewrite andb_false_intro2; auto.
+  simpl. f_equal. f_equal. apply Int64.divs_one.
+  replace Int64.zwordsize with 64; auto. omega.
+Qed.
+
+Theorem divlu_pow2:
+  forall x n logn y,
+  Int64.is_power2' n = Some logn ->
+  divlu x (Vlong n) = Some y ->
+  shrlu x (Vint logn) = y.
+Proof.
+  intros; destruct x; simpl in H0; inv H0.
+  destruct (Int64.eq n Int64.zero); inv H2.
+  simpl.
+  rewrite (Int64.is_power2'_range _ _ H).
+  decEq. symmetry. apply Int64.divu_pow2'. auto.
+Qed.
+
+Theorem divlu_one:
+  forall n, divlu (Vlong n) (Vlong Int64.one) = Some (Vlong n).
+Proof.
+  intros. unfold divlu. rewrite Int64.eq_false; try discriminate.
+  simpl. f_equal. f_equal. apply Int64.divu_one.
+Qed.
+
+Theorem modlu_pow2:
+  forall x n logn y,
+  Int64.is_power2 n = Some logn ->
+  modlu x (Vlong n) = Some y ->
+  andl x (Vlong (Int64.sub n Int64.one)) = y.
+Proof.
+  intros; destruct x; simpl in H0; inv H0.
+  destruct (Int64.eq n Int64.zero); inv H2.
+  simpl. decEq. symmetry. eapply Int64.modu_and; eauto.
+Qed.
+
+Theorem shrxl_carry:
+  forall x y z,
+  shrxl x y = Some z ->
+  addl (shrl x y) (shrl_carry x y) = z.
+Proof.
+  intros. destruct x; destruct y; simpl in H; inv H.
+  destruct (Int.ltu i0 (Int.repr 63)) eqn:?; inv H1.
+  exploit Int.ltu_inv; eauto. change (Int.unsigned (Int.repr 63)) with 63. intros.
+  assert (Int.ltu i0 Int64.iwordsize' = true).
+    unfold Int.ltu. apply zlt_true. change (Int.unsigned Int64.iwordsize') with 64. omega.
+  simpl. rewrite H0. simpl. decEq. rewrite Int64.shrx'_carry; auto.
+Qed.
+
+Theorem shrxl_shrl_2:
+  forall n x z,
+  shrxl x (Vint n) = Some z ->
+  z = (if Int.eq n Int.zero then x else
+         shrl (addl x (shrlu (shrl x (Vint (Int.repr 63)))
+                      (Vint (Int.sub (Int.repr 64) n))))
+              (Vint n)).
+Proof.
+  intros. destruct x; simpl in H; try discriminate.
+  destruct (Int.ltu n (Int.repr 63)) eqn:LT; inv H.
+  exploit Int.ltu_inv; eauto. change (Int.unsigned (Int.repr 63)) with 63; intros LT'.
+  predSpec Int.eq Int.eq_spec n Int.zero.
+- subst n. rewrite Int64.shrx'_zero. auto.
+- simpl. change (Int.ltu (Int.repr 63) Int64.iwordsize') with true. simpl.
+  replace (Int.ltu (Int.sub (Int.repr 64) n) Int64.iwordsize') with true. simpl.
+  replace (Int.ltu n Int64.iwordsize') with true.
+  f_equal; apply Int64.shrx'_shr_2; assumption.
+  symmetry; apply zlt_true. change (Int.unsigned n < 64); omega.
+  symmetry; apply zlt_true. unfold Int.sub. change (Int.unsigned (Int.repr 64)) with 64.
+  assert (Int.unsigned n <> 0). { red; intros; elim H. rewrite <- (Int.repr_unsigned n), H0. auto. }
+  rewrite Int.unsigned_repr.
+  change (Int.unsigned Int64.iwordsize') with 64; omega.
+  assert (64 < Int.max_unsigned) by reflexivity. omega.
 Qed.
 
 Theorem negate_cmp_bool:
@@ -1072,23 +1774,50 @@ Theorem negate_cmpu_bool:
 Proof.
   assert (forall c,
     cmp_different_blocks (negate_comparison c) = option_map negb (cmp_different_blocks c)).
-  destruct c; auto. 
-  destruct x; destruct y; simpl; auto.
-  rewrite Int.negate_cmpu. auto.
-  destruct (Int.eq i Int.zero); auto. 
-  destruct (Int.eq i0 Int.zero); auto.
-  destruct (eq_block b b0).
-  destruct ((valid_ptr b (Int.unsigned i) || valid_ptr b (Int.unsigned i - 1)) &&
-            (valid_ptr b0 (Int.unsigned i0) || valid_ptr b0 (Int.unsigned i0 - 1))).
-  rewrite Int.negate_cmpu. auto.
+  { destruct c; auto. }
+  unfold cmpu_bool; intros; destruct Archi.ptr64 eqn:SF, x, y; auto.
+- rewrite Int.negate_cmpu. auto.
+- rewrite Int.negate_cmpu. auto.
+- destruct (Int.eq i Int.zero && (valid_ptr b (Ptrofs.unsigned i0) || valid_ptr b (Ptrofs.unsigned i0 - 1))); auto.
+- destruct (Int.eq i0 Int.zero && (valid_ptr b (Ptrofs.unsigned i) || valid_ptr b (Ptrofs.unsigned i - 1))); auto.
+- destruct (eq_block b b0).
+  destruct ((valid_ptr b (Ptrofs.unsigned i) || valid_ptr b (Ptrofs.unsigned i - 1)) &&
+            (valid_ptr b0 (Ptrofs.unsigned i0) || valid_ptr b0 (Ptrofs.unsigned i0 - 1))).
+  rewrite Ptrofs.negate_cmpu. auto.
   auto.
-  destruct (valid_ptr b (Int.unsigned i) && valid_ptr b0 (Int.unsigned i0)); auto.
+  destruct (valid_ptr b (Ptrofs.unsigned i) && valid_ptr b0 (Ptrofs.unsigned i0)); auto.
+Qed.
+
+Theorem negate_cmpl_bool:
+  forall c x y, cmpl_bool (negate_comparison c) x y = option_map negb (cmpl_bool c x y).
+Proof.
+  destruct x; destruct y; simpl; auto. rewrite Int64.negate_cmp. auto.
+Qed.
+
+Theorem negate_cmplu_bool:
+  forall valid_ptr c x y,
+  cmplu_bool valid_ptr (negate_comparison c) x y = option_map negb (cmplu_bool valid_ptr c x y).
+Proof.
+  assert (forall c,
+    cmp_different_blocks (negate_comparison c) = option_map negb (cmp_different_blocks c)).
+  { destruct c; auto. }
+  unfold cmplu_bool; intros; destruct Archi.ptr64 eqn:SF, x, y; auto.
+- rewrite Int64.negate_cmpu. auto.
+- simpl. destruct (Int64.eq i Int64.zero && (valid_ptr b (Ptrofs.unsigned i0) || valid_ptr b (Ptrofs.unsigned i0 - 1))); auto.
+- simpl. destruct (Int64.eq i0 Int64.zero && (valid_ptr b (Ptrofs.unsigned i) || valid_ptr b (Ptrofs.unsigned i - 1))); auto.
+- simpl. destruct (eq_block b b0).
+  destruct ((valid_ptr b (Ptrofs.unsigned i) || valid_ptr b (Ptrofs.unsigned i - 1)) &&
+            (valid_ptr b0 (Ptrofs.unsigned i0) || valid_ptr b0 (Ptrofs.unsigned i0 - 1))).
+  rewrite Ptrofs.negate_cmpu. auto.
+  auto.
+  destruct (valid_ptr b (Ptrofs.unsigned i) && valid_ptr b0 (Ptrofs.unsigned i0)); auto.
+- rewrite Int64.negate_cmpu. auto.
 Qed.
 
 Lemma not_of_optbool:
   forall ob, of_optbool (option_map negb ob) = notbool (of_optbool ob).
 Proof.
-  destruct ob; auto. destruct b; auto. 
+  destruct ob; auto. destruct b; auto.
 Qed.
 
 Theorem negate_cmp:
@@ -1118,41 +1847,67 @@ Theorem swap_cmpu_bool:
   cmpu_bool valid_ptr (swap_comparison c) x y =
     cmpu_bool valid_ptr c y x.
 Proof.
-  assert (forall c, cmp_different_blocks (swap_comparison c) = cmp_different_blocks c).
-    destruct c; auto.
-  destruct x; destruct y; simpl; auto.
-  rewrite Int.swap_cmpu. auto.
-  case (Int.eq i Int.zero); auto.
-  case (Int.eq i0 Int.zero); auto.
-  destruct (eq_block b b0); subst.
+  assert (E: forall c, cmp_different_blocks (swap_comparison c) = cmp_different_blocks c).
+  { destruct c; auto. }
+  intros; unfold cmpu_bool. rewrite ! E. destruct Archi.ptr64 eqn:SF, x, y; auto.
+- rewrite Int.swap_cmpu. auto.
+- rewrite Int.swap_cmpu. auto.
+- destruct (eq_block b b0); subst.
   rewrite dec_eq_true.
-  destruct (valid_ptr b0 (Int.unsigned i) || valid_ptr b0 (Int.unsigned i - 1));
-  destruct (valid_ptr b0 (Int.unsigned i0) || valid_ptr b0 (Int.unsigned i0 - 1));
+  destruct (valid_ptr b0 (Ptrofs.unsigned i) || valid_ptr b0 (Ptrofs.unsigned i - 1));
+  destruct (valid_ptr b0 (Ptrofs.unsigned i0) || valid_ptr b0 (Ptrofs.unsigned i0 - 1));
   simpl; auto.
-  rewrite Int.swap_cmpu. auto.
+  rewrite Ptrofs.swap_cmpu. auto.
   rewrite dec_eq_false by auto.
-  destruct (valid_ptr b (Int.unsigned i));
-    destruct (valid_ptr b0 (Int.unsigned i0)); simpl; auto.
+  destruct (valid_ptr b (Ptrofs.unsigned i));
+    destruct (valid_ptr b0 (Ptrofs.unsigned i0)); simpl; auto.
+Qed.
+
+Theorem swap_cmpl_bool:
+  forall c x y,
+  cmpl_bool (swap_comparison c) x y = cmpl_bool c y x.
+Proof.
+  destruct x; destruct y; simpl; auto. rewrite Int64.swap_cmp. auto.
+Qed.
+
+Theorem swap_cmplu_bool:
+  forall valid_ptr c x y,
+  cmplu_bool valid_ptr (swap_comparison c) x y = cmplu_bool valid_ptr c y x.
+Proof.
+  assert (E: forall c, cmp_different_blocks (swap_comparison c) = cmp_different_blocks c).
+  { destruct c; auto. }
+  intros; unfold cmplu_bool. rewrite ! E. destruct Archi.ptr64 eqn:SF, x, y; auto.
+- rewrite Int64.swap_cmpu. auto.
+- destruct (eq_block b b0); subst.
+  rewrite dec_eq_true.
+  destruct (valid_ptr b0 (Ptrofs.unsigned i) || valid_ptr b0 (Ptrofs.unsigned i - 1));
+  destruct (valid_ptr b0 (Ptrofs.unsigned i0) || valid_ptr b0 (Ptrofs.unsigned i0 - 1));
+  simpl; auto.
+  rewrite Ptrofs.swap_cmpu. auto.
+  rewrite dec_eq_false by auto.
+  destruct (valid_ptr b (Ptrofs.unsigned i));
+    destruct (valid_ptr b0 (Ptrofs.unsigned i0)); simpl; auto.
+- rewrite Int64.swap_cmpu. auto.
 Qed.
 
 Theorem negate_cmpf_eq:
   forall v1 v2, notbool (cmpf Cne v1 v2) = cmpf Ceq v1 v2.
 Proof.
-  destruct v1; destruct v2; auto. unfold cmpf, cmpf_bool. 
+  destruct v1; destruct v2; auto. unfold cmpf, cmpf_bool.
   rewrite Float.cmp_ne_eq. destruct (Float.cmp Ceq f f0); auto.
 Qed.
 
 Theorem negate_cmpf_ne:
   forall v1 v2, notbool (cmpf Ceq v1 v2) = cmpf Cne v1 v2.
 Proof.
-  destruct v1; destruct v2; auto. unfold cmpf, cmpf_bool. 
+  destruct v1; destruct v2; auto. unfold cmpf, cmpf_bool.
   rewrite Float.cmp_ne_eq. destruct (Float.cmp Ceq f f0); auto.
 Qed.
 
 Theorem cmpf_le:
   forall v1 v2, cmpf Cle v1 v2 = or (cmpf Clt v1 v2) (cmpf Ceq v1 v2).
 Proof.
-  destruct v1; destruct v2; auto. unfold cmpf, cmpf_bool. 
+  destruct v1; destruct v2; auto. unfold cmpf, cmpf_bool.
   rewrite Float.cmp_le_lt_eq.
   destruct (Float.cmp Clt f f0); destruct (Float.cmp Ceq f f0); auto.
 Qed.
@@ -1160,7 +1915,7 @@ Qed.
 Theorem cmpf_ge:
   forall v1 v2, cmpf Cge v1 v2 = or (cmpf Cgt v1 v2) (cmpf Ceq v1 v2).
 Proof.
-  destruct v1; destruct v2; auto. unfold cmpf, cmpf_bool. 
+  destruct v1; destruct v2; auto. unfold cmpf, cmpf_bool.
   rewrite Float.cmp_ge_gt_eq.
   destruct (Float.cmp Cgt f f0); destruct (Float.cmp Ceq f f0); auto.
 Qed.
@@ -1168,61 +1923,69 @@ Qed.
 Theorem cmp_ne_0_optbool:
   forall ob, cmp Cne (of_optbool ob) (Vint Int.zero) = of_optbool ob.
 Proof.
-  intros. destruct ob; simpl; auto. destruct b; auto. 
+  intros. destruct ob; simpl; auto. destruct b; auto.
 Qed.
 
 Theorem cmp_eq_1_optbool:
   forall ob, cmp Ceq (of_optbool ob) (Vint Int.one) = of_optbool ob.
 Proof.
-  intros. destruct ob; simpl; auto. destruct b; auto. 
+  intros. destruct ob; simpl; auto. destruct b; auto.
 Qed.
 
 Theorem cmp_eq_0_optbool:
   forall ob, cmp Ceq (of_optbool ob) (Vint Int.zero) = of_optbool (option_map negb ob).
 Proof.
-  intros. destruct ob; simpl; auto. destruct b; auto. 
+  intros. destruct ob; simpl; auto. destruct b; auto.
 Qed.
 
 Theorem cmp_ne_1_optbool:
   forall ob, cmp Cne (of_optbool ob) (Vint Int.one) = of_optbool (option_map negb ob).
 Proof.
-  intros. destruct ob; simpl; auto. destruct b; auto. 
+  intros. destruct ob; simpl; auto. destruct b; auto.
 Qed.
 
 Theorem cmpu_ne_0_optbool:
   forall valid_ptr ob,
   cmpu valid_ptr Cne (of_optbool ob) (Vint Int.zero) = of_optbool ob.
 Proof.
-  intros. destruct ob; simpl; auto. destruct b; auto. 
+  intros. destruct ob; simpl; auto. destruct b; auto.
 Qed.
 
 Theorem cmpu_eq_1_optbool:
   forall valid_ptr ob,
   cmpu valid_ptr Ceq (of_optbool ob) (Vint Int.one) = of_optbool ob.
 Proof.
-  intros. destruct ob; simpl; auto. destruct b; auto. 
+  intros. destruct ob; simpl; auto. destruct b; auto.
 Qed.
 
 Theorem cmpu_eq_0_optbool:
   forall valid_ptr ob,
   cmpu valid_ptr Ceq (of_optbool ob) (Vint Int.zero) = of_optbool (option_map negb ob).
 Proof.
-  intros. destruct ob; simpl; auto. destruct b; auto. 
+  intros. destruct ob; simpl; auto. destruct b; auto.
 Qed.
 
 Theorem cmpu_ne_1_optbool:
   forall valid_ptr ob,
   cmpu valid_ptr Cne (of_optbool ob) (Vint Int.one) = of_optbool (option_map negb ob).
 Proof.
-  intros. destruct ob; simpl; auto. destruct b; auto. 
+  intros. destruct ob; simpl; auto. destruct b; auto.
 Qed.
 
 Lemma zero_ext_and:
-  forall n v, 
-  0 < n < Int.zwordsize ->
+  forall n v,
+  0 <= n ->
   Val.zero_ext n v = Val.and v (Vint (Int.repr (two_p n - 1))).
 Proof.
-  intros. destruct v; simpl; auto. decEq. apply Int.zero_ext_and; auto. omega.
+  intros. destruct v; simpl; auto. decEq. apply Int.zero_ext_and; auto.
+Qed.
+
+Lemma zero_ext_andl:
+  forall n v,
+  0 <= n ->
+  Val.zero_ext_l n v = Val.andl v (Vlong (Int64.repr (two_p n - 1))).
+Proof.
+  intros. destruct v; simpl; auto. decEq. apply Int64.zero_ext_and; auto.
 Qed.
 
 Lemma rolm_lt_zero:
@@ -1230,8 +1993,8 @@ Lemma rolm_lt_zero:
 Proof.
   intros. unfold cmp, cmp_bool; destruct v; simpl; auto.
   transitivity (Vint (Int.shru i (Int.repr (Int.zwordsize - 1)))).
-  decEq. symmetry. rewrite Int.shru_rolm. auto. auto. 
-  rewrite Int.shru_lt_zero. destruct (Int.lt i Int.zero); auto. 
+  decEq. symmetry. rewrite Int.shru_rolm. auto. auto.
+  rewrite Int.shru_lt_zero. destruct (Int.lt i Int.zero); auto.
 Qed.
 
 Lemma rolm_ge_zero:
@@ -1242,7 +2005,7 @@ Proof.
   unfold cmp; simpl. destruct (Int.lt i Int.zero); auto.
 Qed.
 
-(** The ``is less defined'' relation between values. 
+(** The ``is less defined'' relation between values.
     A value is less defined than itself, and [Vundef] is
     less defined than any value. *)
 
@@ -1270,15 +2033,21 @@ Inductive lessdef_list: list val -> list val -> Prop :=
       lessdef v1 v2 -> lessdef_list vl1 vl2 ->
       lessdef_list (v1 :: vl1) (v2 :: vl2).
 
-Hint Resolve lessdef_refl lessdef_undef lessdef_list_nil lessdef_list_cons.
+Hint Resolve lessdef_refl lessdef_undef lessdef_list_nil lessdef_list_cons : core.
 
 Lemma lessdef_list_inv:
   forall vl1 vl2, lessdef_list vl1 vl2 -> vl1 = vl2 \/ In Vundef vl1.
 Proof.
   induction 1; simpl.
   tauto.
-  inv H. destruct IHlessdef_list. 
+  inv H. destruct IHlessdef_list.
   left; congruence. tauto. tauto.
+Qed.
+
+Lemma lessdef_list_trans:
+  forall vl1 vl2, lessdef_list vl1 vl2 -> forall vl3, lessdef_list vl2 vl3 -> lessdef_list vl1 vl3.
+Proof.
+  induction 1; intros vl3 LD; inv LD; constructor; eauto using lessdef_trans.
 Qed.
 
 (** Compatibility of operations with the [lessdef] relation. *)
@@ -1315,6 +2084,13 @@ Proof.
   intros. inv H. inv H0. auto. destruct v1'; simpl; auto. simpl; auto.
 Qed.
 
+Lemma addl_lessdef:
+  forall v1 v1' v2 v2',
+  lessdef v1 v1' -> lessdef v2 v2' -> lessdef (addl v1 v2) (addl v1' v2').
+Proof.
+  intros. inv H. inv H0. auto. destruct v1'; simpl; auto. simpl; auto.
+Qed.
+
 Lemma cmpu_bool_lessdef:
   forall valid_ptr valid_ptr' c v1 v1' v2 v2' b,
   (forall b ofs, valid_ptr b ofs = true -> valid_ptr' b ofs = true) ->
@@ -1322,20 +2098,61 @@ Lemma cmpu_bool_lessdef:
   cmpu_bool valid_ptr c v1 v2 = Some b ->
   cmpu_bool valid_ptr' c v1' v2' = Some b.
 Proof.
-  intros. 
-  destruct v1; simpl in H2; try discriminate;
-  destruct v2; simpl in H2; try discriminate;
-  inv H0; inv H1; simpl; auto.
-  destruct (eq_block b0 b1).
-  assert (forall b ofs, valid_ptr b ofs || valid_ptr b (ofs - 1) = true ->
-                        valid_ptr' b ofs || valid_ptr' b (ofs - 1) = true).
-    intros until ofs. rewrite ! orb_true_iff. intuition. 
-  destruct (valid_ptr b0 (Int.unsigned i) || valid_ptr b0 (Int.unsigned i - 1)) eqn:?; try discriminate.
-  destruct (valid_ptr b1 (Int.unsigned i0) || valid_ptr b1 (Int.unsigned i0 - 1)) eqn:?; try discriminate.
-  erewrite !H0 by eauto. auto.
-  destruct (valid_ptr b0 (Int.unsigned i)) eqn:?; try discriminate.
-  destruct (valid_ptr b1 (Int.unsigned i0)) eqn:?; try discriminate.
-  erewrite !H by eauto. auto.
+  intros.
+  assert (X: forall b ofs,
+             valid_ptr b ofs || valid_ptr b (ofs - 1) = true ->
+             valid_ptr' b ofs || valid_ptr' b (ofs - 1) = true).
+  { intros. apply orb_true_intro. destruct (orb_prop _ _ H3).
+    rewrite (H b0 ofs); auto.
+    rewrite (H b0 (ofs - 1)); auto. }
+  inv H0; [ | discriminate].
+  inv H1; [ | destruct v1'; discriminate ].
+  unfold cmpu_bool in *. remember Archi.ptr64 as ptr64.
+  destruct v1'; auto; destruct v2'; auto; destruct ptr64; auto.
+- destruct (Int.eq i Int.zero); auto.
+  destruct (valid_ptr b0 (Ptrofs.unsigned i0) || valid_ptr b0 (Ptrofs.unsigned i0 - 1)) eqn:A; inv H2.
+  rewrite X; auto.
+- destruct (Int.eq i0 Int.zero); auto.
+  destruct (valid_ptr b0 (Ptrofs.unsigned i) || valid_ptr b0 (Ptrofs.unsigned i - 1)) eqn:A; inv H2.
+  rewrite X; auto.
+- destruct (eq_block b0 b1).
++ destruct (valid_ptr b0 (Ptrofs.unsigned i) || valid_ptr b0 (Ptrofs.unsigned i - 1)) eqn:A; inv H2.
+  destruct (valid_ptr b1 (Ptrofs.unsigned i0) || valid_ptr b1 (Ptrofs.unsigned i0 - 1)) eqn:B; inv H1.
+  rewrite ! X; auto.
++ destruct (valid_ptr b0 (Ptrofs.unsigned i) && valid_ptr b1 (Ptrofs.unsigned i0)) eqn:A; inv H2.
+  InvBooleans. rewrite ! H; auto.
+Qed.
+
+Lemma cmplu_bool_lessdef:
+  forall valid_ptr valid_ptr' c v1 v1' v2 v2' b,
+  (forall b ofs, valid_ptr b ofs = true -> valid_ptr' b ofs = true) ->
+  lessdef v1 v1' -> lessdef v2 v2' ->
+  cmplu_bool valid_ptr c v1 v2 = Some b ->
+  cmplu_bool valid_ptr' c v1' v2' = Some b.
+Proof.
+  intros.
+  assert (X: forall b ofs,
+             valid_ptr b ofs || valid_ptr b (ofs - 1) = true ->
+             valid_ptr' b ofs || valid_ptr' b (ofs - 1) = true).
+  { intros. apply orb_true_intro. destruct (orb_prop _ _ H3).
+    rewrite (H b0 ofs); auto.
+    rewrite (H b0 (ofs - 1)); auto. }
+  inv H0; [ | discriminate].
+  inv H1; [ | destruct v1'; discriminate ].
+  unfold cmplu_bool in *. remember Archi.ptr64 as ptr64.
+  destruct v1'; auto; destruct v2'; auto; destruct ptr64; auto.
+- destruct (Int64.eq i Int64.zero); auto.
+  destruct (valid_ptr b0 (Ptrofs.unsigned i0) || valid_ptr b0 (Ptrofs.unsigned i0 - 1)) eqn:A; inv H2.
+  rewrite X; auto.
+- destruct (Int64.eq i0 Int64.zero); auto.
+  destruct (valid_ptr b0 (Ptrofs.unsigned i) || valid_ptr b0 (Ptrofs.unsigned i - 1)) eqn:A; inv H2.
+  rewrite X; auto.
+- destruct (eq_block b0 b1).
++ destruct (valid_ptr b0 (Ptrofs.unsigned i) || valid_ptr b0 (Ptrofs.unsigned i - 1)) eqn:A; inv H2.
+  destruct (valid_ptr b1 (Ptrofs.unsigned i0) || valid_ptr b1 (Ptrofs.unsigned i0 - 1)) eqn:B; inv H1.
+  rewrite ! X; auto.
++ destruct (valid_ptr b0 (Ptrofs.unsigned i) && valid_ptr b1 (Ptrofs.unsigned i0)) eqn:A; inv H2.
+  InvBooleans. rewrite ! H; auto.
 Qed.
 
 Lemma of_optbool_lessdef:
@@ -1343,7 +2160,7 @@ Lemma of_optbool_lessdef:
   (forall b, ob = Some b -> ob' = Some b) ->
   lessdef (of_optbool ob) (of_optbool ob').
 Proof.
-  intros. destruct ob; simpl; auto. rewrite (H b); auto. 
+  intros. destruct ob; simpl; auto. rewrite (H b); auto.
 Qed.
 
 Lemma longofwords_lessdef:
@@ -1356,16 +2173,58 @@ Qed.
 Lemma loword_lessdef:
   forall v v', lessdef v v' -> lessdef (loword v) (loword v').
 Proof.
-  intros. inv H; auto. 
+  intros. inv H; auto.
 Qed.
 
 Lemma hiword_lessdef:
   forall v v', lessdef v v' -> lessdef (hiword v) (hiword v').
 Proof.
-  intros. inv H; auto. 
+  intros. inv H; auto.
 Qed.
 
-End Val.
+Lemma offset_ptr_zero:
+  forall v, lessdef (offset_ptr v Ptrofs.zero) v.
+Proof.
+  intros. destruct v; simpl; auto. rewrite Ptrofs.add_zero; auto.
+Qed.
+
+Lemma offset_ptr_assoc:
+  forall v d1 d2, offset_ptr (offset_ptr v d1) d2 = offset_ptr v (Ptrofs.add d1 d2).
+Proof.
+  intros. destruct v; simpl; auto. f_equal. apply Ptrofs.add_assoc.
+Qed.
+
+Lemma lessdef_normalize:
+  forall v ty, lessdef (normalize v ty) v.
+Proof.
+  intros. destruct v; simpl.
+  - auto.
+  - destruct ty; auto.
+  - destruct ty; auto.
+  - destruct ty; auto.
+  - destruct ty; auto.
+  - destruct ty, Archi.ptr64; auto.
+  - destruct ty; auto.
+    destruct (Archi.vec_typ_eq t v0); auto.
+Qed.
+
+Lemma normalize_lessdef:
+  forall v v' ty, lessdef v v' -> lessdef (normalize v ty) (normalize v' ty).
+Proof.
+  intros. inv H; auto.
+Qed.
+
+Lemma select_lessdef:
+  forall ob ob' v1 v1' v2 v2' ty,
+  ob = None \/ ob = ob' ->
+  lessdef v1 v1' -> lessdef v2 v2' ->
+  lessdef (select ob v1 v2 ty) (select ob' v1' v2' ty).
+Proof.
+  intros; unfold select. destruct H.
+- subst ob; auto.
+- subst ob'; destruct ob as [b|]; auto.
+  apply normalize_lessdef. destruct b; auto.
+Qed.
 
 (** * Values and memory injections *)
 
@@ -1384,73 +2243,130 @@ Definition meminj : Type := block -> option (block * Z).
   as prescribed by the memory injection.  Moreover, [Vundef] values
   inject into any other value. *)
 
-Inductive val_inject (mi: meminj): val -> val -> Prop :=
-  | val_inject_int:
-      forall i, val_inject mi (Vint i) (Vint i)
-  | val_inject_long:
-      forall i, val_inject mi (Vlong i) (Vlong i)
-  | val_inject_int128:
-      forall i, val_inject mi (V128 i) (V128 i)
-  | val_inject_float:
-      forall f, val_inject mi (Vfloat f) (Vfloat f)
-  | val_inject_ptr:
+Inductive inject (mi: meminj): val -> val -> Prop :=
+  | inject_int:
+      forall i, inject mi (Vint i) (Vint i)
+  | inject_long:
+      forall i, inject mi (Vlong i) (Vlong i)
+  | inject_float:
+      forall f, inject mi (Vfloat f) (Vfloat f)
+  | inject_single:
+      forall f, inject mi (Vsingle f) (Vsingle f)
+  | inject_ptr:
       forall b1 ofs1 b2 ofs2 delta,
       mi b1 = Some (b2, delta) ->
-      ofs2 = Int.add ofs1 (Int.repr delta) ->
-      val_inject mi (Vptr b1 ofs1) (Vptr b2 ofs2)
+      ofs2 = Ptrofs.add ofs1 (Ptrofs.repr delta) ->
+      inject mi (Vptr b1 ofs1) (Vptr b2 ofs2)
+  | inject_vec:
+      forall t v, inject mi (Vvec t v) (Vvec t v)
   | val_inject_undef: forall v,
-      val_inject mi Vundef v.
+      inject mi Vundef v.
 
-Hint Constructors val_inject.
+Hint Constructors inject : core.
 
-Inductive val_list_inject (mi: meminj): list val -> list val-> Prop:= 
-  | val_nil_inject :
-      val_list_inject mi nil nil
-  | val_cons_inject : forall v v' vl vl' , 
-      val_inject mi v v' -> val_list_inject mi vl vl'->
-      val_list_inject mi (v :: vl) (v' :: vl').  
+Inductive inject_list (mi: meminj): list val -> list val-> Prop:=
+  | inject_list_nil :
+      inject_list mi nil nil
+  | inject_list_cons : forall v v' vl vl' ,
+      inject mi v v' -> inject_list mi vl vl'->
+      inject_list mi (v :: vl) (v' :: vl').
 
-Hint Resolve val_nil_inject val_cons_inject.
+Hint Resolve inject_list_nil inject_list_cons : core.
+
+Lemma inject_ptrofs:
+  forall mi i, inject mi (Vptrofs i) (Vptrofs i).
+Proof.
+  unfold Vptrofs; intros. destruct Archi.ptr64; auto.
+Qed.
+
+Hint Resolve inject_ptrofs : core.
 
 Section VAL_INJ_OPS.
 
 Variable f: meminj.
 
-Lemma val_load_result_inject:
+Lemma load_result_inject:
   forall chunk v1 v2,
-  val_inject f v1 v2 ->
-  val_inject f (Val.load_result chunk v1) (Val.load_result chunk v2).
+  inject f v1 v2 ->
+  inject f (Val.load_result chunk v1) (Val.load_result chunk v2).
 Proof.
-  intros. inv H; destruct chunk; simpl; econstructor; eauto.
+intros. inv H; destruct chunk; simpl; try constructor; destruct Archi.ptr64; try econstructor; eauto;
+destruct (Archi.vec_typ_eq v0 t); econstructor; eauto.
 Qed.
 
-Remark val_add_inject:
+Remark add_inject:
   forall v1 v1' v2 v2',
-  val_inject f v1 v1' ->
-  val_inject f v2 v2' ->
-  val_inject f (Val.add v1 v2) (Val.add v1' v2').
+  inject f v1 v1' ->
+  inject f v2 v2' ->
+  inject f (Val.add v1 v2) (Val.add v1' v2').
 Proof.
-  intros. inv H; inv H0; simpl; econstructor; eauto.
-  repeat rewrite Int.add_assoc. decEq. apply Int.add_commut.
-  repeat rewrite Int.add_assoc. decEq. apply Int.add_commut.
+  intros. unfold Val.add. destruct Archi.ptr64 eqn:SF.
+- inv H; inv H0; constructor.
+- inv H; inv H0; simpl; auto.
++ econstructor; eauto.
+  rewrite ! Ptrofs.add_assoc. decEq. apply Ptrofs.add_commut.
++ econstructor; eauto.
+  rewrite ! Ptrofs.add_assoc. decEq. apply Ptrofs.add_commut.
 Qed.
 
-Remark val_sub_inject:
+Remark sub_inject:
   forall v1 v1' v2 v2',
-  val_inject f v1 v1' ->
-  val_inject f v2 v2' ->
-  val_inject f (Val.sub v1 v2) (Val.sub v1' v2').
+  inject f v1 v1' ->
+  inject f v2 v2' ->
+  inject f (Val.sub v1 v2) (Val.sub v1' v2').
 Proof.
-  intros. inv H; inv H0; simpl; auto.
-  econstructor; eauto. rewrite Int.sub_add_l. auto.
-  destruct (eq_block b1 b0); auto. subst. rewrite H1 in H. inv H. rewrite dec_eq_true. 
-  rewrite Int.sub_shifted. auto.
+  intros. unfold Val.sub. destruct Archi.ptr64 eqn:SF.
+- inv H; inv H0; constructor.
+- inv H; inv H0; simpl; auto.
++ econstructor; eauto.
+  rewrite Ptrofs.sub_add_l. auto.
++ destruct (eq_block b1 b0); auto.
+  subst. rewrite H1 in H. inv H. rewrite dec_eq_true.
+  rewrite Ptrofs.sub_shifted. auto.
 Qed.
 
-Lemma val_cmp_bool_inject:
+Remark addl_inject:
+  forall v1 v1' v2 v2',
+  inject f v1 v1' ->
+  inject f v2 v2' ->
+  inject f (Val.addl v1 v2) (Val.addl v1' v2').
+Proof.
+  intros. unfold Val.addl. destruct Archi.ptr64 eqn:SF.
+- inv H; inv H0; simpl; auto.
++ econstructor; eauto.
+  rewrite ! Ptrofs.add_assoc. decEq. apply Ptrofs.add_commut.
++ econstructor; eauto.
+  rewrite ! Ptrofs.add_assoc. decEq. apply Ptrofs.add_commut.
+- inv H; inv H0; constructor.
+Qed.
+
+Remark subl_inject:
+  forall v1 v1' v2 v2',
+  inject f v1 v1' ->
+  inject f v2 v2' ->
+  inject f (Val.subl v1 v2) (Val.subl v1' v2').
+Proof.
+  intros. unfold Val.subl. destruct Archi.ptr64 eqn:SF.
+- inv H; inv H0; simpl; auto.
++ econstructor; eauto.
+  rewrite Ptrofs.sub_add_l. auto.
++ destruct (eq_block b1 b0); auto.
+  subst. rewrite H1 in H. inv H. rewrite dec_eq_true.
+  rewrite Ptrofs.sub_shifted. auto.
+- inv H; inv H0; constructor.
+Qed.
+
+Lemma offset_ptr_inject:
+  forall v v' ofs, inject f v v' -> inject f (offset_ptr v ofs) (offset_ptr v' ofs).
+Proof.
+  intros. inv H; simpl; econstructor; eauto.
+  rewrite ! Ptrofs.add_assoc. f_equal. apply Ptrofs.add_commut.
+Qed.
+
+Lemma cmp_bool_inject:
   forall c v1 v2 v1' v2' b,
-  val_inject f v1 v1' ->
-  val_inject f v2 v2' ->
+  inject f v1 v1' ->
+  inject f v2 v2' ->
   Val.cmp_bool c v1 v2 = Some b ->
   Val.cmp_bool c v1' v2' = Some b.
 Proof.
@@ -1465,83 +2381,171 @@ Let weak_valid_ptr2 b ofs := valid_ptr2 b ofs || valid_ptr2 b (ofs - 1).
 Hypothesis valid_ptr_inj:
   forall b1 ofs b2 delta,
   f b1 = Some(b2, delta) ->
-  valid_ptr1 b1 (Int.unsigned ofs) = true ->
-  valid_ptr2 b2 (Int.unsigned (Int.add ofs (Int.repr delta))) = true.
+  valid_ptr1 b1 (Ptrofs.unsigned ofs) = true ->
+  valid_ptr2 b2 (Ptrofs.unsigned (Ptrofs.add ofs (Ptrofs.repr delta))) = true.
 
 Hypothesis weak_valid_ptr_inj:
   forall b1 ofs b2 delta,
   f b1 = Some(b2, delta) ->
-  weak_valid_ptr1 b1 (Int.unsigned ofs) = true ->
-  weak_valid_ptr2 b2 (Int.unsigned (Int.add ofs (Int.repr delta))) = true.
+  weak_valid_ptr1 b1 (Ptrofs.unsigned ofs) = true ->
+  weak_valid_ptr2 b2 (Ptrofs.unsigned (Ptrofs.add ofs (Ptrofs.repr delta))) = true.
 
 Hypothesis weak_valid_ptr_no_overflow:
   forall b1 ofs b2 delta,
   f b1 = Some(b2, delta) ->
-  weak_valid_ptr1 b1 (Int.unsigned ofs) = true ->
-  0 <= Int.unsigned ofs + Int.unsigned (Int.repr delta) <= Int.max_unsigned.
+  weak_valid_ptr1 b1 (Ptrofs.unsigned ofs) = true ->
+  0 <= Ptrofs.unsigned ofs + Ptrofs.unsigned (Ptrofs.repr delta) <= Ptrofs.max_unsigned.
 
 Hypothesis valid_different_ptrs_inj:
   forall b1 ofs1 b2 ofs2 b1' delta1 b2' delta2,
   b1 <> b2 ->
-  valid_ptr1 b1 (Int.unsigned ofs1) = true ->
-  valid_ptr1 b2 (Int.unsigned ofs2) = true ->
+  valid_ptr1 b1 (Ptrofs.unsigned ofs1) = true ->
+  valid_ptr1 b2 (Ptrofs.unsigned ofs2) = true ->
   f b1 = Some (b1', delta1) ->
   f b2 = Some (b2', delta2) ->
   b1' <> b2' \/
-  Int.unsigned (Int.add ofs1 (Int.repr delta1)) <> Int.unsigned (Int.add ofs2 (Int.repr delta2)).
+  Ptrofs.unsigned (Ptrofs.add ofs1 (Ptrofs.repr delta1)) <> Ptrofs.unsigned (Ptrofs.add ofs2 (Ptrofs.repr delta2)).
 
-Lemma val_cmpu_bool_inject:
+Lemma cmpu_bool_inject:
   forall c v1 v2 v1' v2' b,
-  val_inject f v1 v1' ->
-  val_inject f v2 v2' ->
+  inject f v1 v1' ->
+  inject f v2 v2' ->
   Val.cmpu_bool valid_ptr1 c v1 v2 = Some b ->
   Val.cmpu_bool valid_ptr2 c v1' v2' = Some b.
 Proof.
-  Local Opaque Int.add.
-  intros. inv H; simpl in H1; try discriminate; inv H0; simpl in H1; try discriminate; simpl; auto.
-  fold (weak_valid_ptr1 b1 (Int.unsigned ofs1)) in H1.
-  fold (weak_valid_ptr1 b0 (Int.unsigned ofs0)) in H1.
-  fold (weak_valid_ptr2 b2 (Int.unsigned (Int.add ofs1 (Int.repr delta)))).
-  fold (weak_valid_ptr2 b3 (Int.unsigned (Int.add ofs0 (Int.repr delta0)))). 
+  Local Opaque Int.add Ptrofs.add.
+  intros.
+  unfold cmpu_bool in *; destruct Archi.ptr64;
+  inv H; simpl in H1; try discriminate; inv H0; simpl in H1; try discriminate; simpl; auto.
+- fold (weak_valid_ptr1 b1 (Ptrofs.unsigned ofs1)) in H1.
+  fold (weak_valid_ptr2 b2 (Ptrofs.unsigned (Ptrofs.add ofs1 (Ptrofs.repr delta)))).
+  destruct (Int.eq i Int.zero); auto.
+  destruct (weak_valid_ptr1 b1 (Ptrofs.unsigned ofs1)) eqn:E; try discriminate.
+  erewrite weak_valid_ptr_inj by eauto. auto.
+- fold (weak_valid_ptr1 b1 (Ptrofs.unsigned ofs1)) in H1.
+  fold (weak_valid_ptr2 b2 (Ptrofs.unsigned (Ptrofs.add ofs1 (Ptrofs.repr delta)))).
+  destruct (Int.eq i Int.zero); auto.
+  destruct (weak_valid_ptr1 b1 (Ptrofs.unsigned ofs1)) eqn:E; try discriminate.
+  erewrite weak_valid_ptr_inj by eauto. auto.
+- fold (weak_valid_ptr1 b1 (Ptrofs.unsigned ofs1)) in H1.
+  fold (weak_valid_ptr1 b0 (Ptrofs.unsigned ofs0)) in H1.
+  fold (weak_valid_ptr2 b2 (Ptrofs.unsigned (Ptrofs.add ofs1 (Ptrofs.repr delta)))).
+  fold (weak_valid_ptr2 b3 (Ptrofs.unsigned (Ptrofs.add ofs0 (Ptrofs.repr delta0)))).
   destruct (eq_block b1 b0); subst.
   rewrite H in H2. inv H2. rewrite dec_eq_true.
-  destruct (weak_valid_ptr1 b0 (Int.unsigned ofs1)) eqn:?; try discriminate.
-  destruct (weak_valid_ptr1 b0 (Int.unsigned ofs0)) eqn:?; try discriminate.
+  destruct (weak_valid_ptr1 b0 (Ptrofs.unsigned ofs1)) eqn:?; try discriminate.
+  destruct (weak_valid_ptr1 b0 (Ptrofs.unsigned ofs0)) eqn:?; try discriminate.
   erewrite !weak_valid_ptr_inj by eauto. simpl.
-  rewrite <-H1. simpl. decEq. apply Int.translate_cmpu; eauto.
-  destruct (valid_ptr1 b1 (Int.unsigned ofs1)) eqn:?; try discriminate.
-  destruct (valid_ptr1 b0 (Int.unsigned ofs0)) eqn:?; try discriminate.
+  rewrite <-H1. simpl. decEq. apply Ptrofs.translate_cmpu; eauto.
+  destruct (valid_ptr1 b1 (Ptrofs.unsigned ofs1)) eqn:?; try discriminate.
+  destruct (valid_ptr1 b0 (Ptrofs.unsigned ofs0)) eqn:?; try discriminate.
   destruct (eq_block b2 b3); subst.
   assert (valid_ptr_implies: forall b ofs, valid_ptr1 b ofs = true -> weak_valid_ptr1 b ofs = true).
-    intros. unfold weak_valid_ptr1. rewrite H0; auto. 
+    intros. unfold weak_valid_ptr1. rewrite H0; auto.
   erewrite !weak_valid_ptr_inj by eauto using valid_ptr_implies. simpl.
   exploit valid_different_ptrs_inj; eauto. intros [?|?]; [congruence |].
   destruct c; simpl in H1; inv H1.
-  simpl; decEq. rewrite Int.eq_false; auto. congruence.
-  simpl; decEq. rewrite Int.eq_false; auto. congruence.
+  simpl; decEq. rewrite Ptrofs.eq_false; auto. congruence.
+  simpl; decEq. rewrite Ptrofs.eq_false; auto. congruence.
   now erewrite !valid_ptr_inj by eauto.
 Qed.
 
-Lemma val_longofwords_inject:
+Lemma cmplu_bool_inject:
+  forall c v1 v2 v1' v2' b,
+  inject f v1 v1' ->
+  inject f v2 v2' ->
+  Val.cmplu_bool valid_ptr1 c v1 v2 = Some b ->
+  Val.cmplu_bool valid_ptr2 c v1' v2' = Some b.
+Proof.
+  Local Opaque Int64.add Ptrofs.add.
+  intros.
+  unfold cmplu_bool in *; destruct Archi.ptr64;
+  inv H; simpl in H1; try discriminate; inv H0; simpl in H1; try discriminate; simpl; auto.
+- fold (weak_valid_ptr1 b1 (Ptrofs.unsigned ofs1)) in H1.
+  fold (weak_valid_ptr2 b2 (Ptrofs.unsigned (Ptrofs.add ofs1 (Ptrofs.repr delta)))).
+  destruct (Int64.eq i Int64.zero); auto.
+  destruct (weak_valid_ptr1 b1 (Ptrofs.unsigned ofs1)) eqn:E; try discriminate.
+  erewrite weak_valid_ptr_inj by eauto. auto.
+- fold (weak_valid_ptr1 b1 (Ptrofs.unsigned ofs1)) in H1.
+  fold (weak_valid_ptr2 b2 (Ptrofs.unsigned (Ptrofs.add ofs1 (Ptrofs.repr delta)))).
+  destruct (Int64.eq i Int64.zero); auto.
+  destruct (weak_valid_ptr1 b1 (Ptrofs.unsigned ofs1)) eqn:E; try discriminate.
+  erewrite weak_valid_ptr_inj by eauto. auto.
+- fold (weak_valid_ptr1 b1 (Ptrofs.unsigned ofs1)) in H1.
+  fold (weak_valid_ptr1 b0 (Ptrofs.unsigned ofs0)) in H1.
+  fold (weak_valid_ptr2 b2 (Ptrofs.unsigned (Ptrofs.add ofs1 (Ptrofs.repr delta)))).
+  fold (weak_valid_ptr2 b3 (Ptrofs.unsigned (Ptrofs.add ofs0 (Ptrofs.repr delta0)))).
+  destruct (eq_block b1 b0); subst.
+  rewrite H in H2. inv H2. rewrite dec_eq_true.
+  destruct (weak_valid_ptr1 b0 (Ptrofs.unsigned ofs1)) eqn:?; try discriminate.
+  destruct (weak_valid_ptr1 b0 (Ptrofs.unsigned ofs0)) eqn:?; try discriminate.
+  erewrite !weak_valid_ptr_inj by eauto. simpl.
+  rewrite <-H1. simpl. decEq. apply Ptrofs.translate_cmpu; eauto.
+  destruct (valid_ptr1 b1 (Ptrofs.unsigned ofs1)) eqn:?; try discriminate.
+  destruct (valid_ptr1 b0 (Ptrofs.unsigned ofs0)) eqn:?; try discriminate.
+  destruct (eq_block b2 b3); subst.
+  assert (valid_ptr_implies: forall b ofs, valid_ptr1 b ofs = true -> weak_valid_ptr1 b ofs = true).
+    intros. unfold weak_valid_ptr1. rewrite H0; auto.
+  erewrite !weak_valid_ptr_inj by eauto using valid_ptr_implies. simpl.
+  exploit valid_different_ptrs_inj; eauto. intros [?|?]; [congruence |].
+  destruct c; simpl in H1; inv H1.
+  simpl; decEq. rewrite Ptrofs.eq_false; auto. congruence.
+  simpl; decEq. rewrite Ptrofs.eq_false; auto. congruence.
+  now erewrite !valid_ptr_inj by eauto.
+Qed.
+
+Lemma longofwords_inject:
   forall v1 v2 v1' v2',
-  val_inject f v1 v1' -> val_inject f v2 v2' -> val_inject f (Val.longofwords v1 v2) (Val.longofwords v1' v2').
+  inject f v1 v1' -> inject f v2 v2' -> inject f (Val.longofwords v1 v2) (Val.longofwords v1' v2').
 Proof.
   intros. unfold Val.longofwords. inv H; auto. inv H0; auto.
 Qed.
 
-Lemma val_loword_inject:
-  forall v v', val_inject f v v' -> val_inject f (Val.loword v) (Val.loword v').
+Lemma loword_inject:
+  forall v v', inject f v v' -> inject f (Val.loword v) (Val.loword v').
 Proof.
-  intros. unfold Val.loword; inv H; auto. 
+  intros. unfold Val.loword; inv H; auto.
 Qed.
 
-Lemma val_hiword_inject:
-  forall v v', val_inject f v v' -> val_inject f (Val.hiword v) (Val.hiword v').
+Lemma hiword_inject:
+  forall v v', inject f v v' -> inject f (Val.hiword v) (Val.hiword v').
 Proof.
-  intros. unfold Val.hiword; inv H; auto. 
+  intros. unfold Val.hiword; inv H; auto.
+Qed.
+
+Lemma normalize_inject:
+  forall v v' ty, inject f v v' -> inject f (normalize v ty) (normalize v' ty).
+Proof.
+  intros. inv H.
+- destruct ty; constructor.
+- destruct ty; constructor.
+- destruct ty; constructor.
+- destruct ty; constructor.
+- simpl; destruct ty; auto.
++ destruct Archi.ptr64; econstructor; eauto.
++ destruct Archi.ptr64; econstructor; eauto.
+- simpl; destruct ty; auto.
++ destruct (Archi.vec_typ_eq t v); econstructor; eauto.
+- simpl; destruct ty; auto.
+Qed.
+
+Lemma select_inject:
+  forall ob ob' v1 v1' v2 v2' ty,
+  ob = None \/ ob = ob' ->
+  inject f v1 v1' -> inject f v2 v2' ->
+  inject f (select ob v1 v2 ty) (select ob' v1' v2' ty).
+Proof.
+  intros; unfold select. destruct H.
+- subst ob; auto.
+- subst ob'; destruct ob as [b|]; auto.
+  apply normalize_inject. destruct b; auto.
 Qed.
 
 End VAL_INJ_OPS.
+
+End Val.
+
+Notation meminj := Val.meminj.
 
 (** Monotone evolution of a memory injection. *)
 
@@ -1553,42 +2557,42 @@ Lemma inject_incr_refl :
 Proof. unfold inject_incr. auto. Qed.
 
 Lemma inject_incr_trans :
-  forall f1 f2 f3, 
+  forall f1 f2 f3,
   inject_incr f1 f2 -> inject_incr f2 f3 -> inject_incr f1 f3 .
 Proof.
-  unfold inject_incr; intros. eauto. 
+  unfold inject_incr; intros. eauto.
 Qed.
 
 Lemma val_inject_incr:
   forall f1 f2 v v',
   inject_incr f1 f2 ->
-  val_inject f1 v v' ->
-  val_inject f2 v v'.
+  Val.inject f1 v v' ->
+  Val.inject f2 v v'.
 Proof.
   intros. inv H0; eauto.
 Qed.
 
-Lemma val_list_inject_incr:
+Lemma val_inject_list_incr:
   forall f1 f2 vl vl' ,
-  inject_incr f1 f2 -> val_list_inject f1 vl vl' ->
-  val_list_inject f2 vl vl'.
+  inject_incr f1 f2 -> Val.inject_list f1 vl vl' ->
+  Val.inject_list f2 vl vl'.
 Proof.
   induction vl; intros; inv H0. auto.
   constructor. eapply val_inject_incr; eauto. auto.
 Qed.
 
-Hint Resolve inject_incr_refl val_inject_incr val_list_inject_incr.
+Hint Resolve inject_incr_refl val_inject_incr val_inject_list_incr : core.
 
 Lemma val_inject_lessdef:
-  forall v1 v2, Val.lessdef v1 v2 <-> val_inject (fun b => Some(b, 0)) v1 v2.
+  forall v1 v2, Val.lessdef v1 v2 <-> Val.inject (fun b => Some(b, 0)) v1 v2.
 Proof.
   intros; split; intros.
-  inv H; auto. destruct v2; econstructor; eauto. rewrite Int.add_zero; auto. 
-  inv H; auto. inv H0. rewrite Int.add_zero; auto.
+  inv H; auto. destruct v2; econstructor; eauto. rewrite Ptrofs.add_zero; auto.
+  inv H; auto. inv H0. rewrite Ptrofs.add_zero; auto.
 Qed.
 
-Lemma val_list_inject_lessdef:
-  forall vl1 vl2, Val.lessdef_list vl1 vl2 <-> val_list_inject (fun b => Some(b, 0)) vl1 vl2.
+Lemma val_inject_list_lessdef:
+  forall vl1 vl2, Val.lessdef_list vl1 vl2 <-> Val.inject_list (fun b => Some(b, 0)) vl1 vl2.
 Proof.
   intros; split.
   induction 1; constructor; auto. apply val_inject_lessdef; auto.
@@ -1601,12 +2605,12 @@ Definition inject_id : meminj := fun b => Some(b, 0).
 
 Lemma val_inject_id:
   forall v1 v2,
-  val_inject inject_id v1 v2 <-> Val.lessdef v1 v2.
+  Val.inject inject_id v1 v2 <-> Val.lessdef v1 v2.
 Proof.
   intros; split; intros.
-  inv H; auto. 
-  unfold inject_id in H0. inv H0. rewrite Int.add_zero. constructor.
-  inv H. destruct v2; econstructor. unfold inject_id; reflexivity. rewrite Int.add_zero; auto.
+  inv H; auto.
+  unfold inject_id in H0. inv H0. rewrite Ptrofs.add_zero. constructor.
+  inv H. destruct v2; econstructor. unfold inject_id; reflexivity. rewrite Ptrofs.add_zero; auto.
   constructor.
 Qed.
 
@@ -1625,10 +2629,13 @@ Definition compose_meminj (f f': meminj) : meminj :=
 
 Lemma val_inject_compose:
   forall f f' v1 v2 v3,
-  val_inject f v1 v2 -> val_inject f' v2 v3 ->
-  val_inject (compose_meminj f f') v1 v3.
+  Val.inject f v1 v2 -> Val.inject f' v2 v3 ->
+  Val.inject (compose_meminj f f') v1 v3.
 Proof.
   intros. inv H; auto; inv H0; auto. econstructor.
-  unfold compose_meminj; rewrite H1; rewrite H3; eauto. 
-  rewrite Int.add_assoc. decEq. unfold Int.add. apply Int.eqm_samerepr. auto with ints.
-Qed. 
+  unfold compose_meminj; rewrite H1; rewrite H3; eauto.
+  rewrite Ptrofs.add_assoc. decEq. unfold Ptrofs.add. apply Ptrofs.eqm_samerepr. auto with ints.
+  apply Eqdep_dec.inj_pair2_eq_dec in H2.
+   rewrite H2; econstructor.
+  exact Archi.vec_typ_eq.
+Qed.
