ccomp-simd/lib/Coqlib.v
@@ -17,10 +17,13 @@
     used throughout the development.  It complements the Coq standard
     library. *)
 
+Require Export String.
 Require Export ZArith.
 Require Export Znumtheory.
 Require Export List.
 Require Export Bool.
+
+Global Set Asymmetric Patterns.
 
 (** * Useful tactics *)
 
@@ -30,7 +33,7 @@ Ltac predSpec pred predspec x y :=
   generalize (predspec x y); case (pred x y); intro.
 
 Ltac caseEq name :=
-  generalize (refl_equal name); pattern name at -1 in |- *; case name.
+  generalize (eq_refl name); pattern name at -1 in |- *; case name.
 
 Ltac destructEq name :=
   destruct name eqn:?.
@@ -107,14 +110,14 @@ Proof.
   intros. case (peq x y); intros.
   elim H; auto.
   auto.
-Qed.  
+Qed.
 
 Definition Plt: positive -> positive -> Prop := Pos.lt.
 
 Lemma Plt_ne:
   forall (x y: positive), Plt x y -> x <> y.
 Proof.
-  unfold Plt; intros. red; intro. subst y. eelim Pos.lt_irrefl; eauto. 
+  unfold Plt; intros. red; intro. subst y. eelim Pos.lt_irrefl; eauto.
 Qed.
 Hint Resolve Plt_ne: coqlib.
 
@@ -123,23 +126,23 @@ Lemma Plt_trans:
 Proof (Pos.lt_trans).
 
 Lemma Plt_succ:
-  forall (x: positive), Plt x (Psucc x).
+  forall (x: positive), Plt x (Pos.succ x).
 Proof.
-  unfold Plt; intros. apply Pos.lt_succ_r. apply Pos.le_refl. 
+  unfold Plt; intros. apply Pos.lt_succ_r. apply Pos.le_refl.
 Qed.
 Hint Resolve Plt_succ: coqlib.
 
 Lemma Plt_trans_succ:
-  forall (x y: positive), Plt x y -> Plt x (Psucc y).
+  forall (x y: positive), Plt x y -> Plt x (Pos.succ y).
 Proof.
   intros. apply Plt_trans with y. assumption. apply Plt_succ.
 Qed.
 Hint Resolve Plt_succ: coqlib.
 
 Lemma Plt_succ_inv:
-  forall (x y: positive), Plt x (Psucc y) -> Plt x y \/ x = y.
+  forall (x y: positive), Plt x (Pos.succ y) -> Plt x y \/ x = y.
 Proof.
-  unfold Plt; intros. rewrite Pos.lt_succ_r in H. 
+  unfold Plt; intros. rewrite Pos.lt_succ_r in H.
   apply Pos.le_lteq; auto.
 Qed.
 
@@ -163,7 +166,7 @@ Proof (Pos.le_trans).
 Lemma Plt_Ple: forall (p q: positive), Plt p q -> Ple p q.
 Proof (Pos.lt_le_incl).
 
-Lemma Ple_succ: forall (p: positive), Ple p (Psucc p).
+Lemma Ple_succ: forall (p: positive), Ple p (Pos.succ p).
 Proof.
   intros. apply Plt_Ple. apply Plt_succ.
 Qed.
@@ -186,7 +189,7 @@ Section POSITIVE_ITERATION.
 
 Lemma Plt_wf: well_founded Plt.
 Proof.
-  apply well_founded_lt_compat with nat_of_P.
+  apply well_founded_lt_compat with Pos.to_nat.
   intros. apply nat_of_P_lt_Lt_compare_morphism. exact H.
 Qed.
 
@@ -195,16 +198,16 @@ Variable v1: A.
 Variable f: positive -> A -> A.
 
 Lemma Ppred_Plt:
-  forall x, x <> xH -> Plt (Ppred x) x.
+  forall x, x <> xH -> Plt (Pos.pred x) x.
 Proof.
-  intros. elim (Psucc_pred x); intro. contradiction.
-  set (y := Ppred x) in *. rewrite <- H0. apply Plt_succ.
+  intros. elim (Pos.succ_pred_or x); intro. contradiction.
+  set (y := Pos.pred x) in *. rewrite <- H0. apply Plt_succ.
 Qed.
 
 Let iter (x: positive) (P: forall y, Plt y x -> A) : A :=
   match peq x xH with
   | left EQ => v1
-  | right NOTEQ => f (Ppred x) (P (Ppred x) (Ppred_Plt x NOTEQ))
+  | right NOTEQ => f (Pos.pred x) (P (Pos.pred x) (Ppred_Plt x NOTEQ))
   end.
 
 Definition positive_rec : positive -> A :=
@@ -226,27 +229,27 @@ Proof.
 Qed.
 
 Lemma positive_rec_succ:
-  forall x, positive_rec (Psucc x) = f x (positive_rec x).
+  forall x, positive_rec (Pos.succ x) = f x (positive_rec x).
 Proof.
   intro. rewrite unroll_positive_rec. unfold iter.
-  case (peq (Psucc x) 1); intro.
+  case (peq (Pos.succ x) 1); intro.
   destruct x; simpl in e; discriminate.
-  rewrite Ppred_succ. auto.
+  rewrite Pos.pred_succ. auto.
 Qed.
 
 Lemma positive_Peano_ind:
   forall (P: positive -> Prop),
   P xH ->
-  (forall x, P x -> P (Psucc x)) ->
+  (forall x, P x -> P (Pos.succ x)) ->
   forall x, P x.
 Proof.
   intros.
   apply (well_founded_ind Plt_wf P).
-  intros. 
+  intros.
   case (peq x0 xH); intro.
   subst x0; auto.
-  elim (Psucc_pred x0); intro. contradiction. rewrite <- H2.
-  apply H0. apply H1. apply Ppred_Plt. auto. 
+  elim (Pos.succ_pred_or x0); intro. contradiction. rewrite <- H2.
+  apply H0. apply H1. apply Ppred_Plt. auto.
 Qed.
 
 End POSITIVE_ITERATION.
@@ -269,14 +272,14 @@ Proof.
   intros. case (zeq x y); intros.
   elim H; auto.
   auto.
-Qed.  
+Qed.
 
 Open Scope Z_scope.
 
 Definition zlt: forall (x y: Z), {x < y} + {x >= y} := Z_lt_dec.
 
 Lemma zlt_true:
-  forall (A: Type) (x y: Z) (a b: A), 
+  forall (A: Type) (x y: Z) (a b: A),
   x < y -> (if zlt x y then a else b) = a.
 Proof.
   intros. case (zlt x y); intros.
@@ -285,7 +288,7 @@ Proof.
 Qed.
 
 Lemma zlt_false:
-  forall (A: Type) (x y: Z) (a b: A), 
+  forall (A: Type) (x y: Z) (a b: A),
   x >= y -> (if zlt x y then a else b) = b.
 Proof.
   intros. case (zlt x y); intros.
@@ -296,7 +299,7 @@ Qed.
 Definition zle: forall (x y: Z), {x <= y} + {x > y} := Z_le_gt_dec.
 
 Lemma zle_true:
-  forall (A: Type) (x y: Z) (a b: A), 
+  forall (A: Type) (x y: Z) (a b: A),
   x <= y -> (if zle x y then a else b) = a.
 Proof.
   intros. case (zle x y); intros.
@@ -305,7 +308,7 @@ Proof.
 Qed.
 
 Lemma zle_false:
-  forall (A: Type) (x y: Z) (a b: A), 
+  forall (A: Type) (x y: Z) (a b: A),
   x > y -> (if zle x y then a else b) = b.
 Proof.
   intros. case (zle x y); intros.
@@ -325,17 +328,17 @@ Proof.
 Qed.
 
 Lemma two_power_nat_two_p:
-  forall x, two_power_nat x = two_p (Z_of_nat x).
+  forall x, two_power_nat x = two_p (Z.of_nat x).
 Proof.
-  induction x. auto. 
-  rewrite two_power_nat_S. rewrite inj_S. rewrite two_p_S. omega. omega.
+  induction x. auto.
+  rewrite two_power_nat_S. rewrite Nat2Z.inj_succ. rewrite two_p_S. omega. omega.
 Qed.
 
 Lemma two_p_monotone:
   forall x y, 0 <= x <= y -> two_p x <= two_p y.
 Proof.
   intros.
-  replace (two_p x) with (two_p x * 1) by omega. 
+  replace (two_p x) with (two_p x * 1) by omega.
   replace y with (x + (y - x)) by omega.
   rewrite two_p_is_exp; try omega.
   apply Zmult_le_compat_l.
@@ -348,7 +351,7 @@ Lemma two_p_monotone_strict:
 Proof.
   intros. assert (two_p x <= two_p (y - 1)). apply two_p_monotone; omega.
   assert (two_p (y - 1) > 0). apply two_p_gt_ZERO. omega.
-  replace y with (Zsucc (y - 1)) by omega. rewrite two_p_S. omega. omega.
+  replace y with (Z.succ (y - 1)) by omega. rewrite two_p_S. omega. omega.
 Qed.
 
 Lemma two_p_strict:
@@ -356,7 +359,7 @@ Lemma two_p_strict:
 Proof.
   intros x0 GT. pattern x0. apply natlike_ind.
   simpl. omega.
-  intros. rewrite two_p_S; auto. generalize (two_p_gt_ZERO x H). omega. 
+  intros. rewrite two_p_S; auto. generalize (two_p_gt_ZERO x H). omega.
   omega.
 Qed.
 
@@ -366,91 +369,61 @@ Proof.
   intros. assert (x = 0 \/ x - 1 >= 0) by omega. destruct H0.
   subst. vm_compute. auto.
   replace (two_p x) with (2 * two_p (x - 1)).
-  generalize (two_p_strict _ H0). omega. 
+  generalize (two_p_strict _ H0). omega.
   rewrite <- two_p_S. decEq. omega. omega.
 Qed.
 
 (** Properties of [Zmin] and [Zmax] *)
 
 Lemma Zmin_spec:
-  forall x y, Zmin x y = if zlt x y then x else y.
+  forall x y, Z.min x y = if zlt x y then x else y.
 Proof.
-  intros. case (zlt x y); unfold Zlt, Zge; intro z.
-  unfold Zmin. rewrite z. auto.
-  unfold Zmin. caseEq (x ?= y); intro. 
-  apply Zcompare_Eq_eq. auto.
+  intros. case (zlt x y); unfold Z.lt, Z.ge; intro z.
+  unfold Z.min. rewrite z. auto.
+  unfold Z.min. caseEq (x ?= y); intro.
+  apply Z.compare_eq. auto.
   contradiction.
   reflexivity.
 Qed.
 
 Lemma Zmax_spec:
-  forall x y, Zmax x y = if zlt y x then x else y.
+  forall x y, Z.max x y = if zlt y x then x else y.
 Proof.
-  intros. case (zlt y x); unfold Zlt, Zge; intro z.
-  unfold Zmax. rewrite <- (Zcompare_antisym y x).
+  intros. case (zlt y x); unfold Z.lt, Z.ge; intro z.
+  unfold Z.max. rewrite <- (Zcompare_antisym y x).
   rewrite z. simpl. auto.
-  unfold Zmax. rewrite <- (Zcompare_antisym y x).
+  unfold Z.max. rewrite <- (Zcompare_antisym y x).
   caseEq (y ?= x); intro; simpl.
-  symmetry. apply Zcompare_Eq_eq. auto.
+  symmetry. apply Z.compare_eq. auto.
   contradiction. reflexivity.
 Qed.
 
 Lemma Zmax_bound_l:
-  forall x y z, x <= y -> x <= Zmax y z.
+  forall x y z, x <= y -> x <= Z.max y z.
 Proof.
-  intros. generalize (Zmax1 y z). omega.
+  intros. generalize (Z.le_max_l y z). omega.
 Qed.
 Lemma Zmax_bound_r:
-  forall x y z, x <= z -> x <= Zmax y z.
+  forall x y z, x <= z -> x <= Z.max y z.
 Proof.
-  intros. generalize (Zmax2 y z). omega.
+  intros. generalize (Z.le_max_r y z). omega.
 Qed.
 
 (** Properties of Euclidean division and modulus. *)
-
-Lemma Zdiv_small:
-  forall x y, 0 <= x < y -> x / y = 0.
-Proof.
-  intros. assert (y > 0). omega. 
-  assert (forall a b,
-    0 <= a < y ->
-    0 <= y * b + a < y ->
-    b = 0).
-  intros. 
-  assert (b = 0 \/ b > 0 \/ (-b) > 0). omega.
-  elim H3; intro.
-  auto.
-  elim H4; intro.
-  assert (y * b >= y * 1). apply Zmult_ge_compat_l. omega. omega. 
-  omegaContradiction. 
-  assert (y * (-b) >= y * 1). apply Zmult_ge_compat_l. omega. omega.
-  rewrite <- Zopp_mult_distr_r in H6. omegaContradiction.
-  apply H1 with (x mod y). 
-  apply Z_mod_lt. auto.
-  rewrite <- Z_div_mod_eq. auto. auto.
-Qed.
-
-Lemma Zmod_small:
-  forall x y, 0 <= x < y -> x mod y = x.
-Proof.
-  intros. assert (y > 0). omega.
-  generalize (Z_div_mod_eq x y H0). 
-  rewrite (Zdiv_small x y H). omega.
-Qed.
 
 Lemma Zmod_unique:
   forall x y a b,
   x = a * y + b -> 0 <= b < y -> x mod y = b.
 Proof.
-  intros. subst x. rewrite Zplus_comm. 
-  rewrite Z_mod_plus. apply Zmod_small. auto. omega.
+  intros. subst x. rewrite Z.add_comm.
+  rewrite Z_mod_plus. apply Z.mod_small. auto. omega.
 Qed.
 
 Lemma Zdiv_unique:
   forall x y a b,
   x = a * y + b -> 0 <= b < y -> x / y = a.
 Proof.
-  intros. subst x. rewrite Zplus_comm.
+  intros. subst x. rewrite Z.add_comm.
   rewrite Z_div_plus. rewrite (Zdiv_small b y H0). omega. omega.
 Qed.
 
@@ -458,30 +431,7 @@ Lemma Zdiv_Zdiv:
   forall a b c,
   b > 0 -> c > 0 -> (a / b) / c = a / (b * c).
 Proof.
-  intros.
-  generalize (Z_div_mod_eq a b H). generalize (Z_mod_lt a b H). intros.
-  generalize (Z_div_mod_eq (a/b) c H0). generalize (Z_mod_lt (a/b) c H0). intros.
-  set (q1 := a / b) in *. set (r1 := a mod b) in *.
-  set (q2 := q1 / c) in *. set (r2 := q1 mod c) in *.
-  symmetry. apply Zdiv_unique with (r2 * b + r1). 
-  rewrite H2. rewrite H4. ring.
-  split. 
-  assert (0 <= r2 * b). apply Zmult_le_0_compat. omega. omega. omega.
-  assert ((r2 + 1) * b <= c * b).
-  apply Zmult_le_compat_r. omega. omega. 
-  replace ((r2 + 1) * b) with (r2 * b + b) in H5 by ring.
-  replace (c * b) with (b * c) in H5 by ring.
-  omega.
-Qed.
-
-Lemma Zmult_le_compat_l_neg :
-  forall n m p:Z, n >= m -> p <= 0 -> p * n <= p * m.
-Proof.
-  intros.
-  assert ((-p) * n >= (-p) * m). apply Zmult_ge_compat_l. auto. omega.
-  replace (p * n) with (- ((-p) * n)) by ring.
-  replace (p * m) with (- ((-p) * m)) by ring.
-  omega.
+  intros. apply Z.div_div; omega.
 Qed.
 
 Lemma Zdiv_interval_1:
@@ -490,17 +440,17 @@ Lemma Zdiv_interval_1:
   lo * b <= a < hi * b ->
   lo <= a/b < hi.
 Proof.
-  intros. 
+  intros.
   generalize (Z_div_mod_eq a b H1). generalize (Z_mod_lt a b H1). intros.
   set (q := a/b) in *. set (r := a mod b) in *.
   split.
   assert (lo < (q + 1)).
-  apply Zmult_lt_reg_r with b. omega.  
-  apply Zle_lt_trans with a. omega. 
+  apply Zmult_lt_reg_r with b. omega.
+  apply Z.le_lt_trans with a. omega.
   replace ((q + 1) * b) with (b * q + b) by ring.
   omega.
   omega.
-  apply Zmult_lt_reg_r with b. omega. 
+  apply Zmult_lt_reg_r with b. omega.
   replace (q * b) with (b * q) by ring.
   omega.
 Qed.
@@ -513,9 +463,9 @@ Proof.
   intros.
   assert (lo <= a / b < hi+1).
   apply Zdiv_interval_1. omega. omega. auto.
-  assert (lo * b <= lo * 1). apply Zmult_le_compat_l_neg. omega. omega. 
+  assert (lo * b <= lo * 1) by (apply Z.mul_le_mono_nonpos_l; omega).
   replace (lo * 1) with lo in H3 by ring.
-  assert ((hi + 1) * 1 <= (hi + 1) * b). apply Zmult_le_compat_l. omega. omega.
+  assert ((hi + 1) * 1 <= (hi + 1) * b) by (apply Z.mul_le_mono_nonneg_l; omega).
   replace ((hi + 1) * 1) with (hi + 1) in H4 by ring.
   omega.
   omega.
@@ -526,90 +476,36 @@ Lemma Zmod_recombine:
   a > 0 -> b > 0 ->
   x mod (a * b) = ((x/b) mod a) * b + (x mod b).
 Proof.
-  intros. 
-  set (xb := x/b). 
-  apply Zmod_unique with (xb/a).
-  generalize (Z_div_mod_eq x b H0); fold xb; intro EQ1.
-  generalize (Z_div_mod_eq xb a H); intro EQ2.
-  rewrite EQ2 in EQ1. 
-  eapply trans_eq. eexact EQ1. ring.
-  generalize (Z_mod_lt x b H0). intro. 
-  generalize (Z_mod_lt xb a H). intro.
-  assert (0 <= xb mod a * b <= a * b - b).
-    split. apply Zmult_le_0_compat; omega.
-    replace (a * b - b) with ((a - 1) * b) by ring.
-    apply Zmult_le_compat; omega. 
-  omega.
+  intros. rewrite (Z.mul_comm a b). rewrite Z.rem_mul_r by omega. ring. 
 Qed.
 
 (** Properties of divisibility. *)
-
-Lemma Zdivides_trans:
-  forall x y z, (x | y) -> (y | z) -> (x | z).
-Proof.
-  intros x y z [a A] [b B]; subst. exists (a*b); ring.
-Qed.
-
-Definition Zdivide_dec:
-  forall (p q: Z), p > 0 -> { (p|q) } + { ~(p|q) }.
-Proof.
-  intros. destruct (zeq (Zmod q p) 0).
-  left. exists (q / p). 
-  transitivity (p * (q / p) + (q mod p)). apply Z_div_mod_eq; auto.
-  transitivity (p * (q / p)). omega. ring.
-  right; red; intros. elim n. apply Z_div_exact_1; auto. 
-  inv H0. rewrite Z_div_mult; auto. ring.
-Defined.
-Global Opaque Zdivide_dec.
 
 Lemma Zdivide_interval:
   forall a b c,
   0 < c -> 0 <= a < b -> (c | a) -> (c | b) -> 0 <= a <= b - c.
 Proof.
   intros. destruct H1 as [x EQ1]. destruct H2 as [y EQ2]. subst. destruct H0.
-  split. omega. exploit Zmult_lt_reg_r; eauto. intros. 
+  split. omega. exploit Zmult_lt_reg_r; eauto. intros.
   replace (y * c - c) with ((y - 1) * c) by ring.
   apply Zmult_le_compat_r; omega.
 Qed.
 
 (** Conversion from [Z] to [nat]. *)
 
-Definition nat_of_Z: Z -> nat := Z.to_nat.
-
-Lemma nat_of_Z_of_nat:
-  forall n, nat_of_Z (Z_of_nat n) = n.
+Lemma Z_to_nat_neg:
+  forall n, n <= 0 -> Z.to_nat n = O.
 Proof.
-  exact Nat2Z.id.
+  destruct n; unfold Z.le; simpl; auto. congruence.
 Qed.
 
-Lemma nat_of_Z_max:
-  forall z, Z_of_nat (nat_of_Z z) = Zmax z 0.
+Lemma Z_to_nat_max:
+  forall z, Z.of_nat (Z.to_nat z) = Z.max z 0.
 Proof.
-  intros. unfold Zmax. destruct z; simpl; auto. 
-  change (Z.of_nat (Z.to_nat (Zpos p)) = Zpos p).
-  apply Z2Nat.id. compute; intuition congruence. 
+  intros. destruct (zle 0 z).
+- rewrite Z2Nat.id by auto. xomega.
+- rewrite Z_to_nat_neg by omega. xomega.
 Qed.
-
-Lemma nat_of_Z_eq:
-  forall z, z >= 0 -> Z_of_nat (nat_of_Z z) = z.
-Proof.
-  unfold nat_of_Z; intros. apply Z2Nat.id. omega.
-Qed.
-
-Lemma nat_of_Z_neg:
-  forall n, n <= 0 -> nat_of_Z n = O.
-Proof.
-  destruct n; unfold Zle; simpl; auto. congruence.
-Qed.
-
-Lemma nat_of_Z_plus:
-  forall p q,
-  p >= 0 -> q >= 0 ->
-  nat_of_Z (p + q) = (nat_of_Z p + nat_of_Z q)%nat.
-Proof.
-  unfold nat_of_Z; intros. apply Z2Nat.inj_add; omega. 
-Qed.
-
 
 (** Alignment: [align n amount] returns the smallest multiple of [amount]
   greater than or equal to [n]. *)
@@ -619,17 +515,17 @@ Definition align (n: Z) (amount: Z) :=
 
 Lemma align_le: forall x y, y > 0 -> x <= align x y.
 Proof.
-  intros. unfold align. 
+  intros. unfold align.
   generalize (Z_div_mod_eq (x + y - 1) y H). intro.
-  replace ((x + y - 1) / y * y) 
+  replace ((x + y - 1) / y * y)
      with ((x + y - 1) - (x + y - 1) mod y).
   generalize (Z_mod_lt (x + y - 1) y H). omega.
-  rewrite Zmult_comm. omega.
+  rewrite Z.mul_comm. omega.
 Qed.
 
 Lemma align_divides: forall x y, y > 0 -> (y | align x y).
 Proof.
-  intros. unfold align. apply Zdivide_factor_l. 
+  intros. unfold align. apply Z.divide_factor_r.
 Qed.
 
 Lemma divides_align_eq: forall x y,
@@ -638,14 +534,15 @@ Proof.
 intros.
 destruct (Z.eq_dec y 0).
  subst; unfold align.
- rewrite Z.add_0_l. cutrewrite ((x - 1) / x = 0); [omega|].
- apply Zdiv_small. omega.
+ rewrite Z.add_0_l. 
+ enough ((x - 1) / x = 0) as ->; [omega|].
+ apply Zdiv_small; omega.
 destruct H1 as [z Hz]; rewrite Hz.
 unfold align.
-cutrewrite (z * x + x - 1 = z * x + (x - 1)); [|ring].
+enough (z * x + x - 1 = z * x + (x - 1)) as -> ; [|ring].
 rewrite Z_div_plus_full_l;[|omega].
 ring_simplify.
-cutrewrite ((x - 1) / x = 0);[omega|].
+enough ((x - 1) / x = 0) as ->;[omega|].
 apply Zdiv_small; omega.
 Qed.
 
@@ -659,6 +556,12 @@ Definition option_eq (A: Type) (eqA: forall (x y: A), {x=y} + {x<>y}):
   forall (x y: option A), {x=y} + {x<>y}.
 Proof. decide equality. Defined.
 Global Opaque option_eq.
+
+(** Lifting a relation to an option type. *)
+
+Inductive option_rel (A B: Type) (R: A -> B -> Prop) : option A -> option B -> Prop :=
+  | option_rel_none: option_rel R None None
+  | option_rel_some: forall x y, R x y -> option_rel R (Some x) (Some y).
 
 (** Mapping a function over an option type. *)
 
@@ -706,7 +609,7 @@ Hint Resolve nth_error_nil: coqlib.
 Fixpoint list_length_z_aux (A: Type) (l: list A) (acc: Z) {struct l}: Z :=
   match l with
   | nil => acc
-  | hd :: tl => list_length_z_aux tl (Zsucc acc)
+  | hd :: tl => list_length_z_aux tl (Z.succ acc)
   end.
 
 Remark list_length_z_aux_shift:
@@ -715,7 +618,7 @@ Remark list_length_z_aux_shift:
 Proof.
   induction l; intros; simpl.
   omega.
-  replace (n - m) with (Zsucc n - Zsucc m) by omega. auto.
+  replace (n - m) with (Z.succ n - Z.succ m) by omega. auto.
 Qed.
 
 Definition list_length_z (A: Type) (l: list A) : Z :=
@@ -726,14 +629,14 @@ Lemma list_length_z_cons:
   list_length_z (hd :: tl) = list_length_z tl + 1.
 Proof.
   intros. unfold list_length_z. simpl.
-  rewrite (list_length_z_aux_shift tl 1 0). omega. 
+  rewrite (list_length_z_aux_shift tl 1 0). omega.
 Qed.
 
 Lemma list_length_z_pos:
   forall (A: Type) (l: list A),
   list_length_z l >= 0.
 Proof.
-  induction l; simpl. unfold list_length_z; simpl. omega. 
+  induction l; simpl. unfold list_length_z; simpl. omega.
   rewrite list_length_z_cons. omega.
 Qed.
 
@@ -742,7 +645,7 @@ Lemma list_length_z_map:
   list_length_z (map f l) = list_length_z l.
 Proof.
   induction l. reflexivity. simpl. repeat rewrite list_length_z_cons. congruence.
-Qed. 
+Qed.
 
 (** Extract the n-th element of a list, as [List.nth_error] does,
     but the index [n] is of type [Z]. *)
@@ -750,14 +653,14 @@ Qed.
 Fixpoint list_nth_z (A: Type) (l: list A) (n: Z) {struct l}: option A :=
   match l with
   | nil => None
-  | hd :: tl => if zeq n 0 then Some hd else list_nth_z tl (Zpred n)
+  | hd :: tl => if zeq n 0 then Some hd else list_nth_z tl (Z.pred n)
   end.
 
 Lemma list_nth_z_in:
   forall (A: Type) (l: list A) n x,
   list_nth_z l n = Some x -> In x l.
 Proof.
-  induction l; simpl; intros. 
+  induction l; simpl; intros.
   congruence.
   destruct (zeq n 0). left; congruence. right; eauto.
 Qed.
@@ -779,7 +682,7 @@ Proof.
   discriminate.
   rewrite list_length_z_cons. destruct (zeq n 0).
   generalize (list_length_z_pos l); omega.
-  exploit IHl; eauto. unfold Zpred. omega. 
+  exploit IHl; eauto. omega.
 Qed.
 
 (** Properties of [List.incl] (list inclusion). *)
@@ -812,7 +715,7 @@ Lemma incl_same_head:
   forall (A: Type) (x: A) (l1 l2: list A),
   incl l1 l2 -> incl (x::l1) (x::l2).
 Proof.
-  intros; red; simpl; intros. intuition. 
+  intros; red; simpl; intros. intuition.
 Qed.
 
 (** Properties of [List.map] (mapping a function over a list). *)
@@ -865,9 +768,9 @@ Lemma list_in_map_inv:
 Proof.
   induction l; simpl; intros.
   contradiction.
-  elim H; intro. 
+  elim H; intro.
   exists a; intuition auto.
-  generalize (IHl y H0). intros [x [EQ IN]]. 
+  generalize (IHl y H0). intros [x [EQ IN]].
   exists x; tauto.
 Qed.
 
@@ -886,8 +789,8 @@ Lemma list_append_map_inv:
 Proof.
   induction m1; simpl; intros.
   exists (@nil A); exists l; auto.
-  destruct l; simpl in H; inv H. 
-  exploit IHm1; eauto. intros [l1 [l2 [P [Q R]]]]. subst l. 
+  destruct l; simpl in H; inv H.
+  exploit IHm1; eauto. intros [l1 [l2 [P [Q R]]]]. subst l.
   exists (a0 :: l1); exists l2; intuition. simpl; congruence.
 Qed.
 
@@ -914,7 +817,7 @@ Remark list_fold_left_app:
   forall l1 l2 accu,
   list_fold_left accu (l1 ++ l2) = list_fold_left (list_fold_left accu l1) l2.
 Proof.
-  induction l1; simpl; intros. 
+  induction l1; simpl; intros.
   auto.
   rewrite IHl1. auto.
 Qed.
@@ -924,11 +827,11 @@ Lemma list_fold_right_eq:
   list_fold_right l base =
   match l with nil => base | x :: l' => f x (list_fold_right l' base) end.
 Proof.
-  unfold list_fold_right; intros. 
+  unfold list_fold_right; intros.
   destruct l.
   auto.
-  unfold rev'. rewrite <- ! rev_alt. simpl.  
-  rewrite list_fold_left_app. simpl. auto. 
+  unfold rev'. rewrite <- ! rev_alt. simpl.
+  rewrite list_fold_left_app. simpl. auto.
 Qed.
 
 Lemma list_fold_right_spec:
@@ -960,7 +863,7 @@ Proof.
   intros. apply in_or_app; simpl. elim (in_app_or _ _ _ H); intro; auto.
 Qed.
 
-(** [list_disjoint l1 l2] holds iff [l1] and [l2] have no elements 
+(** [list_disjoint l1 l2] holds iff [l1] and [l2] have no elements
   in common. *)
 
 Definition list_disjoint (A: Type) (l1 l2: list A) : Prop :=
@@ -984,21 +887,21 @@ Lemma list_disjoint_cons_left:
   forall (A: Type) (a: A) (l1 l2: list A),
   list_disjoint (a :: l1) l2 -> list_disjoint l1 l2.
 Proof.
-  unfold list_disjoint; simpl; intros. apply H; tauto. 
+  unfold list_disjoint; simpl; intros. apply H; tauto.
 Qed.
 
 Lemma list_disjoint_cons_right:
   forall (A: Type) (a: A) (l1 l2: list A),
   list_disjoint l1 (a :: l2) -> list_disjoint l1 l2.
 Proof.
-  unfold list_disjoint; simpl; intros. apply H; tauto. 
+  unfold list_disjoint; simpl; intros. apply H; tauto.
 Qed.
 
 Lemma list_disjoint_notin:
   forall (A: Type) (l1 l2: list A) (a: A),
   list_disjoint l1 l2 -> In a l1 -> ~(In a l2).
 Proof.
-  unfold list_disjoint; intros; red; intros. 
+  unfold list_disjoint; intros; red; intros.
   apply H with a a; auto.
 Qed.
 
@@ -1006,8 +909,8 @@ Lemma list_disjoint_sym:
   forall (A: Type) (l1 l2: list A),
   list_disjoint l1 l2 -> list_disjoint l2 l1.
 Proof.
-  unfold list_disjoint; intros. 
-  apply sym_not_equal. apply H; auto.
+  unfold list_disjoint; intros.
+  apply not_eq_sym. apply H; auto.
 Qed.
 
 Lemma list_disjoint_dec:
@@ -1017,9 +920,9 @@ Proof.
   induction l1; intros.
   left; red; intros. elim H.
   case (In_dec eqA_dec a l2); intro.
-  right; red; intro. apply (H a a); auto with coqlib. 
+  right; red; intro. apply (H a a); auto with coqlib.
   case (IHl1 l2); intro.
-  left; red; intros. elim H; intro. 
+  left; red; intros. elim H; intro.
     red; intro; subst a y. contradiction.
     apply l; auto.
   right; red; intros. elim n0. eapply list_disjoint_cons_left; eauto.
@@ -1046,9 +949,9 @@ Lemma list_norepet_dec:
 Proof.
   induction l.
   left; constructor.
-  destruct IHl. 
+  destruct IHl.
   case (In_dec eqA_dec a l); intro.
-  right. red; intro. inversion H. contradiction. 
+  right. red; intro. inversion H. contradiction.
   left. constructor; auto.
   right. red; intro. inversion H. contradiction.
 Defined.
@@ -1064,7 +967,7 @@ Proof.
   constructor.
   red; intro. generalize (list_in_map_inv f _ _ H2).
   intros [x [EQ IN]]. generalize EQ. change (f hd <> f x).
-  apply H1. tauto. tauto. 
+  apply H1. tauto. tauto.
   red; intro; subst x. contradiction.
   apply IHlist_norepet. intros. apply H1. tauto. tauto. auto.
 Qed.
@@ -1074,20 +977,20 @@ Remark list_norepet_append_commut:
   list_norepet (a ++ b) -> list_norepet (b ++ a).
 Proof.
   intro A.
-  assert (forall (x: A) (b: list A) (a: list A), 
-           list_norepet (a ++ b) -> ~(In x a) -> ~(In x b) -> 
+  assert (forall (x: A) (b: list A) (a: list A),
+           list_norepet (a ++ b) -> ~(In x a) -> ~(In x b) ->
            list_norepet (a ++ x :: b)).
     induction a; simpl; intros.
     constructor; auto.
     inversion H. constructor. red; intro.
     elim (in_app_or _ _ _ H6); intro.
     elim H4. apply in_or_app. tauto.
-    elim H7; intro. subst a. elim H0. left. auto. 
+    elim H7; intro. subst a. elim H0. left. auto.
     elim H4. apply in_or_app. tauto.
     auto.
   induction a; simpl; intros.
   rewrite <- app_nil_end. auto.
-  inversion H0. apply H. auto. 
+  inversion H0. apply H. auto.
   red; intro; elim H3. apply in_or_app. tauto.
   red; intro; elim H3. apply in_or_app. tauto.
 Qed.
@@ -1102,10 +1005,10 @@ Proof.
   tauto.
   inversion H; subst. rewrite IHl1 in H3. rewrite in_app in H2.
   intuition.
-  constructor; auto. red; intros. elim H2; intro. congruence. auto. 
-  destruct H as [B [C D]]. inversion B; subst. 
-  constructor. rewrite in_app. intuition. elim (D a a); auto. apply in_eq. 
-  rewrite IHl1. intuition. red; intros. apply D; auto. apply in_cons; auto. 
+  constructor; auto. red; intros. elim H2; intro. congruence. auto.
+  destruct H as [B [C D]]. inversion B; subst.
+  constructor. rewrite in_app. intuition. elim (D a a); auto. apply in_eq.
+  rewrite IHl1. intuition. red; intros. apply D; auto. apply in_cons; auto.
 Qed.
 
 Lemma list_norepet_append:
@@ -1150,7 +1053,7 @@ Lemma is_tail_cons_left:
   forall (A: Type) (i: A) c1 c2, is_tail (i :: c1) c2 -> is_tail c1 c2.
 Proof.
   induction c2; intros; inversion H.
-  constructor. constructor. constructor. auto. 
+  constructor. constructor. constructor. auto.
 Qed.
 
 Hint Resolve is_tail_refl is_tail_cons is_tail_in is_tail_cons_left: coqlib.
@@ -1188,10 +1091,10 @@ Inductive list_forall2: list A -> list B -> Prop :=
 
 Lemma list_forall2_app:
   forall a2 b2 a1 b1,
-  list_forall2 a1 b1 -> list_forall2 a2 b2 -> 
+  list_forall2 a1 b1 -> list_forall2 a2 b2 ->
   list_forall2 (a1 ++ a2) (b1 ++ b2).
 Proof.
-  induction 1; intros; simpl. auto. constructor; auto. 
+  induction 1; intros; simpl. auto. constructor; auto.
 Qed.
 
 Lemma list_forall2_length:
@@ -1199,6 +1102,24 @@ Lemma list_forall2_length:
   list_forall2 l1 l2 -> length l1 = length l2.
 Proof.
   induction 1; simpl; congruence.
+Qed.
+
+Lemma list_forall2_in_left:
+  forall x1 l1 l2,
+  list_forall2 l1 l2 -> In x1 l1 -> exists x2, In x2 l2 /\ P x1 x2.
+Proof.
+  induction 1; simpl; intros. contradiction. destruct H1.
+  subst; exists b1; auto.
+  exploit IHlist_forall2; eauto. intros (x2 & U & V); exists x2; auto.
+Qed.
+
+Lemma list_forall2_in_right:
+  forall x2 l1 l2,
+  list_forall2 l1 l2 -> In x2 l2 -> exists x1, In x1 l1 /\ P x1 x2.
+Proof.
+  induction 1; simpl; intros. contradiction. destruct H1.
+  subst; exists a1; auto.
+  exploit IHlist_forall2; eauto. intros (x1 & U & V); exists x1; auto.
 Qed.
 
 End FORALL2.
@@ -1212,7 +1133,7 @@ Lemma list_forall2_imply:
 Proof.
   induction 1; intros.
   constructor.
-  constructor. auto with coqlib. apply IHlist_forall2; auto. 
+  constructor. auto with coqlib. apply IHlist_forall2; auto.
   intros. auto with coqlib.
 Qed.
 
@@ -1227,7 +1148,7 @@ Fixpoint list_drop (A: Type) (n: nat) (x: list A) {struct n} : list A :=
 Lemma list_drop_incl:
   forall (A: Type) (x: A) n (l: list A), In x (list_drop n l) -> In x l.
 Proof.
-  induction n; simpl; intros. auto. 
+  induction n; simpl; intros. auto.
   destruct l; auto with coqlib.
 Qed.
 
@@ -1242,7 +1163,7 @@ Lemma list_map_drop:
   forall (A B: Type) (f: A -> B) n (l: list A),
   list_drop n (map f l) = map f (list_drop n l).
 Proof.
-  induction n; simpl; intros. auto. 
+  induction n; simpl; intros. auto.
   destruct l; simpl; auto.
 Qed.
 
@@ -1268,10 +1189,8 @@ Qed.
 
 (** * Definitions and theorems over boolean types *)
 
-Definition proj_sumbool (P Q: Prop) (a: {P} + {Q}) : bool :=
+Definition proj_sumbool {P Q: Prop} (a: {P} + {Q}) : bool :=
   if a then true else false.
-
-Implicit Arguments proj_sumbool [P Q].
 
 Coercion proj_sumbool: sumbool >-> bool.
 
@@ -1284,7 +1203,7 @@ Qed.
 Lemma proj_sumbool_is_true:
   forall (P: Prop) (a: {P}+{~P}), P -> proj_sumbool a = true.
 Proof.
-  intros. unfold proj_sumbool. destruct a. auto. contradiction. 
+  intros. unfold proj_sumbool. destruct a. auto. contradiction.
 Qed.
 
 Ltac InvBooleans :=
@@ -1323,7 +1242,7 @@ Lemma dec_eq_sym:
   (if dec_eq x y then ifso else ifnot) =
   (if dec_eq y x then ifso else ifnot).
 Proof.
-  intros. destruct (dec_eq x y). 
+  intros. destruct (dec_eq x y).
   subst y. rewrite dec_eq_true. auto.
   rewrite dec_eq_false; auto.
 Qed.
@@ -1369,22 +1288,22 @@ Inductive lex_ord: A*B -> A*B -> Prop :=
   | lex_ord_right: forall a b1 b2,
       ordB b1 b2 -> lex_ord (a,b1) (a,b2).
 
-Lemma wf_lex_ord: 
+Lemma wf_lex_ord:
   well_founded ordA -> well_founded ordB -> well_founded lex_ord.
 Proof.
   intros Awf Bwf.
   assert (forall a, Acc ordA a -> forall b, Acc ordB b -> Acc lex_ord (a, b)).
     induction 1. induction 1. constructor; intros. inv H3.
     apply H0. auto. apply Bwf.
-    apply H2; auto. 
+    apply H2; auto.
   red; intros. destruct a as [a b]. apply H; auto.
 Qed.
 
 Lemma transitive_lex_ord:
   transitive _ ordA -> transitive _ ordB -> transitive _ lex_ord.
 Proof.
-  intros trA trB; red; intros. 
-  inv H; inv H0. 
+  intros trA trB; red; intros.
+  inv H; inv H0.
   left; eapply trA; eauto.
   left; auto.
   left; auto.
@@ -1393,3 +1312,34 @@ Qed.
 
 End LEX_ORDER.
 
+(** * Nonempty lists *)
+
+Inductive nlist (A: Type) : Type :=
+  | nbase: A -> nlist A
+  | ncons: A -> nlist A -> nlist A.
+
+Definition nfirst {A: Type} (l: nlist A) :=
+  match l with nbase a => a | ncons a l' => a end.
+
+Fixpoint nlast {A: Type} (l: nlist A) :=
+  match l with nbase a => a | ncons a l' => nlast l' end.
+
+Fixpoint nIn {A: Type} (x: A) (l: nlist A) : Prop :=
+  match l with
+  | nbase a => a = x
+  | ncons a l => a = x \/ nIn x l
+  end.
+
+Inductive nlist_forall2 {A B: Type} (R: A -> B -> Prop) : nlist A -> nlist B -> Prop :=
+  | nbase_forall2: forall a b, R a b -> nlist_forall2 R (nbase a) (nbase b)
+  | ncons_forall2: forall a l b m, R a b -> nlist_forall2 R l m -> nlist_forall2 R (ncons a l) (ncons b m).
+
+Lemma nlist_forall2_imply:
+  forall (A B: Type) (P1: A -> B -> Prop) (l1: nlist A) (l2: nlist B),
+  nlist_forall2 P1 l1 l2 ->
+  forall (P2: A -> B -> Prop),
+  (forall v1 v2, nIn v1 l1 -> nIn v2 l2 -> P1 v1 v2 -> P2 v1 v2) ->
+  nlist_forall2 P2 l1 l2.
+Proof.
+  induction 1; simpl; intros; constructor; auto.
+Qed.
