ccomp-simd/x86_64/Archi.v
@@ -1,0 +1,159 @@
+(* *********************************************************************)
+(*                                                                     *)
+(*              The Compcert verified compiler                         *)
+(*                                                                     *)
+(*                Xavier Leroy, INRIA Paris                            *)
+(*                Jacques-Henri Jourdan, INRIA Paris                   *)
+(*                                                                     *)
+(*  Copyright Institut National de Recherche en Informatique et en     *)
+(*  Automatique.  All rights reserved.  This file is distributed       *)
+(*  under the terms of the GNU General Public License as published by  *)
+(*  the Free Software Foundation, either version 2 of the License, or  *)
+(*  (at your option) any later version.  This file is also distributed *)
+(*  under the terms of the INRIA Non-Commercial License Agreement.     *)
+(*                                                                     *)
+(* *********************************************************************)
+
+(** Architecture-dependent parameters for x86 in 64-bit mode *)
+
+Require Import ZArith List.
+(*From Flocq*)
+Require Import Binary Bits.
+
+Definition ptr64 := true.
+
+Definition big_endian := false.
+
+Definition align_int64 := 8%Z.
+Definition align_float64 := 8%Z.
+
+Definition splitlong := negb ptr64.
+
+Lemma splitlong_ptr32: splitlong = true -> ptr64 = false.
+Proof.
+  unfold splitlong. destruct ptr64; simpl; congruence.
+Qed.
+
+Definition default_nan_64 := (true, iter_nat 51 _ xO xH).
+Definition default_nan_32 := (true, iter_nat 22 _ xO xH).
+
+(* Always choose the first NaN argument, if any *)
+
+Definition choose_nan_64 (l: list (bool * positive)) : bool * positive :=
+  match l with nil => default_nan_64 | n :: _ => n end.
+
+Definition choose_nan_32 (l: list (bool * positive)) : bool * positive :=
+  match l with nil => default_nan_32 | n :: _ => n end.
+
+Lemma choose_nan_64_idem: forall n,
+  choose_nan_64 (n :: n :: nil) = choose_nan_64 (n :: nil).
+Proof. auto. Qed.
+
+Lemma choose_nan_32_idem: forall n,
+  choose_nan_32 (n :: n :: nil) = choose_nan_32 (n :: nil).
+Proof. auto. Qed.
+
+Definition fma_order {A: Type} (x y z: A) := (x, y, z).
+
+Definition fma_invalid_mul_is_nan := false.
+
+Definition float_of_single_preserves_sNaN := false.
+
+Global Opaque ptr64 big_endian splitlong
+              default_nan_64 choose_nan_64
+              default_nan_32 choose_nan_32
+              fma_order fma_invalid_mul_is_nan
+              float_of_single_preserves_sNaN.
+
+
+(** SIMD support *)
+
+Inductive vec_typ : Type :=
+ | T128		(**r 128bit wide vectores *)
+ | T256.        (**r 256bit wide vectores *)
+
+Lemma vec_typ_eq: forall (t1 t2: vec_typ), {t1=t2} + {t1<>t2}.
+Proof. decide equality. Defined.
+
+(** Type rank of vector extensions *)
+Definition vec_typ_rnk ty :=
+ match ty with
+ | T128 => 2
+ | T256 => 3
+ end.
+
+(*
+Inductive vec_chunk :=
+ | M128		(**r 128bit wide memory chunk *)
+ | M256.	(**r 256bit wide memory chunk *)
+
+Definition vec_type_of_chunk (c:vec_chunk) : vec_typ :=
+ match c with
+ | M128 => T128
+ | M256 => T256
+ end.
+
+Definition vec_chunk_of_type (ty:vec_typ) : vec_chunk :=
+ match ty with
+ | T128 => M128
+ | T256 => M256
+ end.
+*)
+
+
+
+(*
+(* remark: typesize is specified in 32bit units (to be compatible
+  with Locations.v *)
+Definition vec_typesize (t:vec_variant) : Z := 4.
+
+Lemma vec_typesize_pos: forall t, vec_typesize t > 0.
+Proof. destruct t; unfold vec_typesize; omega. Qed.
+
+Definition vec_variant_sem (t:vec_variant) : Type := Int128.int.
+
+Definition vec_intval {t} (v:vec_variant_sem t) : Z := Int128.unsigned v.
+
+Definition vec_repr {t} (v:Z) : vec_variant_sem t := Int128.repr v.
+
+(* for the sake of somplicity, we consider a chunk-definition
+ for each of the vec-variants available...
+Definition vec_chunk : Type := unit.
+
+Definition vec_type_of_chunk (c:vec_chunk) : vec_variant := tt.
+Definition vec_chunk_of_type (c:vec_variant) : vec_chunk := tt.
+*)
+
+(* alignment is specified in bytes --- we adopt the same alignment
+ as for Tfloat *)
+Definition vec_align_chunk (t:vec_variant) : Z := align_float64.
+
+(*Notation align_vec128 := 16%Z (only parsing).*)
+
+Lemma vec_align_chunk_pos: forall t, vec_align_chunk t > 0.
+Proof. destruct t; unfold vec_align_chunk; omega. Qed.
+
+Lemma vec_align_le_divides: forall t, 
+  (vec_align_chunk t | 4 * vec_typesize t).
+Proof.
+destruct t; unfold vec_align_chunk, vec_typesize; simpl.
+exists 2; omega.
+Qed.
+
+(** [vec_low_off] should be [x-1] when [x] is the size of the second
+  biggest slot-size *)
+Definition vec_low_off := 7.
+
+Definition vec_widest := tt.
+
+Hint Unfold vec_widest vec_low_off.
+
+(** remark: [vec_variant_index] should be monotonic wrt [typesize] *)
+Definition vec_variant_index (t:vec_variant) : positive := 1%positive.
+
+
+(** Homogeneous aggregates maximum size *)
+Definition hom_fstruct_size := 4%nat.
+*)
+
+
