ccomp-simd/x86_64/ArchiVec.v
@@ -1,0 +1,63 @@
+(** Architecture-dependent parameters for x86 in 64-bit mode *)
+
+Require Import ZArith List.
+
+Open Scope Z_scope.
+
+Require Import Archi Integers AST.
+
+Definition vec_typ_sem (t:vec_typ) : Type :=
+ match t with
+ | T128 => Int128.int
+ | T256 => Int256.int
+ end.
+
+Definition vec_intval {t}: vec_typ_sem t -> Z :=
+ match t with
+ | T128 => Int128.unsigned
+ | T256 => Int256.unsigned
+ end.
+
+Definition vec_repr {t}: Z -> vec_typ_sem t :=
+ match t with
+ | T128 => Int128.repr
+ | T256 => Int256.repr
+ end.
+
+Lemma vec_eq (ty: vec_typ): forall (x y: vec_typ_sem ty), {x=y} + {x<>y}.
+Proof.
+destruct ty; unfold vec_typ_sem; intros.
+- apply Int128.eq_dec.
+- apply Int256.eq_dec.
+Qed.
+
+(*
+Definition vec_typ_align (t:vec_typ) : Z := 4 * two_power_nat (vec_typ_rnk t).
+
+Lemma vec_align_chunk_pos: forall t, vec_typ_align t > 0.
+Proof. destruct t; unfold vec_typ_align; omega. Qed.
+
+Lemma vec_align_le_divides: forall t, 
+  (vec_align_chunk t | 4 * vec_typesize t).
+Proof.
+destruct t; unfold vec_align_chunk, vec_typesize; simpl.
+exists 2; omega.
+Qed.
+
+(** [vec_low_off] should be [x-1] when [x] is the size of the second
+  biggest slot-size *)
+Definition vec_low_off := 7.
+
+Definition vec_widest := tt.
+
+Hint Unfold vec_widest vec_low_off.
+
+(** remark: [vec_variant_index] should be monotonic wrt [typesize] *)
+Definition vec_variant_index (t:vec_variant) : positive := 1%positive.
+
+
+(** Homogeneous aggregates maximum size *)
+Definition hom_fstruct_size := 4%nat.
+*)
+
+
